@prefix ex: <http://www.huawei.com/ontology/> .
@prefix owl: <http://www.w3.org/2002/07/owl#> .
@prefix prov: <http://www.w3.org/ns/prov#> .
@prefix rdfs: <http://www.w3.org/2000/01/rdf-schema#> .
@prefix sh: <http://www.w3.org/ns/shacl#> .
@prefix xsd: <http://www.w3.org/2001/XMLSchema#> .

ex:alarm-state a sh:NodeShape ;
    rdfs:label "alarm-state" ;
    sh:datatype rdfs:Literal .

ex:as-number a sh:NodeShape ;
    rdfs:label "as-number" ;
    sh:datatype xsd:unsignedInt .

ex:counter32 a sh:NodeShape ;
    rdfs:label "counter32" ;
    sh:datatype xsd:unsignedInt .

ex:counter64 a sh:NodeShape ;
    rdfs:label "counter64" ;
    sh:datatype xsd:unsignedLong .

ex:date-and-time a sh:NodeShape ;
    rdfs:label "date-and-time" ;
    sh:datatype xsd:string ;
    sh:pattern "\\d{4}-\\d{2}-\\d{2}T\\d{2}:\\d{2}:\\d{2}(\\.\\d+)?(Z|[\\+\\-]\\d{2}:\\d{2})" .

ex:domain-name a sh:NodeShape ;
    rdfs:label "domain-name" ;
    sh:datatype xsd:string ;
    sh:maxLength 253 ;
    sh:minLength 1 ;
    sh:pattern "((([a-zA-Z0-9_]([a-zA-Z0-9\\-_]){0,61})?[a-zA-Z0-9]\\.)*([a-zA-Z0-9_]([a-zA-Z0-9\\-_]){0,61})?[a-zA-Z0-9]\\.?)|\\." .

ex:dotted-quad a sh:NodeShape ;
    rdfs:label "dotted-quad" ;
    sh:datatype xsd:string ;
    sh:pattern "(([0-9]|[1-9][0-9]|1[0-9][0-9]|2[0-4][0-9]|25[0-5])\\.){3}([0-9]|[1-9][0-9]|1[0-9][0-9]|2[0-4][0-9]|25[0-5])" .

ex:dscp a sh:NodeShape ;
    rdfs:label "dscp" ;
    sh:datatype xsd:unsignedByte ;
    sh:maxInclusive 63 ;
    sh:minInclusive 0 .

ex:gauge32 a sh:NodeShape ;
    rdfs:label "gauge32" ;
    sh:datatype xsd:unsignedInt .

ex:gauge64 a sh:NodeShape ;
    rdfs:label "gauge64" ;
    sh:datatype xsd:unsignedLong .

ex:hex-string a sh:NodeShape ;
    rdfs:label "hex-string" ;
    sh:datatype xsd:string ;
    sh:pattern "([0-9a-fA-F]{2}(:[0-9a-fA-F]{2})*)?" .

<http://www.huawei.com/ontology/identity/ATB> a owl:Class,
        owl:NamedIndividual ;
    rdfs:label "ATB" ;
    rdfs:comment "Access Terminal Box." ;
    rdfs:subClassOf <http://www.huawei.com/ontology/identity/passive-device-type> ;
    prov:wasDerivedFrom "nwi-passive:ATB?identity" .

<http://www.huawei.com/ontology/identity/FAT> a owl:Class,
        owl:NamedIndividual ;
    rdfs:label "FAT" ;
    rdfs:comment "Fiber Access Terminal." ;
    rdfs:subClassOf <http://www.huawei.com/ontology/identity/passive-device-type> ;
    prov:wasDerivedFrom "nwi-passive:FAT?identity" .

<http://www.huawei.com/ontology/identity/FDT> a owl:Class,
        owl:NamedIndividual ;
    rdfs:label "FDT" ;
    rdfs:comment "Fiber Distribution Terminal." ;
    rdfs:subClassOf <http://www.huawei.com/ontology/identity/passive-device-type> ;
    prov:wasDerivedFrom "nwi-passive:FDT?identity" .

<http://www.huawei.com/ontology/identity/G652A> a owl:Class,
        owl:NamedIndividual ;
    rdfs:label "G652A" ;
    rdfs:comment "ITU-T G.652A fiber." ;
    rdfs:subClassOf <http://www.huawei.com/ontology/identity/fiber-type> ;
    prov:wasDerivedFrom "nwi-passive:G652A?identity" .

<http://www.huawei.com/ontology/identity/G652B> a owl:Class,
        owl:NamedIndividual ;
    rdfs:label "G652B" ;
    rdfs:comment "ITU-T G.652B fiber." ;
    rdfs:subClassOf <http://www.huawei.com/ontology/identity/fiber-type> ;
    prov:wasDerivedFrom "nwi-passive:G652B?identity" .

<http://www.huawei.com/ontology/identity/G652C> a owl:Class,
        owl:NamedIndividual ;
    rdfs:label "G652C" ;
    rdfs:comment "ITU-T G.652C fiber." ;
    rdfs:subClassOf <http://www.huawei.com/ontology/identity/fiber-type> ;
    prov:wasDerivedFrom "nwi-passive:G652C?identity" .

<http://www.huawei.com/ontology/identity/G652D> a owl:Class,
        owl:NamedIndividual ;
    rdfs:label "G652D" ;
    rdfs:comment "ITU-T G.652D fiber." ;
    rdfs:subClassOf <http://www.huawei.com/ontology/identity/fiber-type> ;
    prov:wasDerivedFrom "nwi-passive:G652D?identity" .

<http://www.huawei.com/ontology/identity/G653> a owl:Class,
        owl:NamedIndividual ;
    rdfs:label "G653" ;
    rdfs:comment "ITU-T G.653 fiber." ;
    rdfs:subClassOf <http://www.huawei.com/ontology/identity/fiber-type> ;
    prov:wasDerivedFrom "nwi-passive:G653?identity" .

<http://www.huawei.com/ontology/identity/G654> a owl:Class,
        owl:NamedIndividual ;
    rdfs:label "G654" ;
    rdfs:comment "ITU-T G.654 fiber." ;
    rdfs:subClassOf <http://www.huawei.com/ontology/identity/fiber-type> ;
    prov:wasDerivedFrom "nwi-passive:G654?identity" .

<http://www.huawei.com/ontology/identity/G655> a owl:Class,
        owl:NamedIndividual ;
    rdfs:label "G655" ;
    rdfs:comment "ITU-T G.655 fiber." ;
    rdfs:subClassOf <http://www.huawei.com/ontology/identity/fiber-type> ;
    prov:wasDerivedFrom "nwi-passive:G655?identity" .

<http://www.huawei.com/ontology/identity/G656> a owl:Class,
        owl:NamedIndividual ;
    rdfs:label "G656" ;
    rdfs:comment "ITU-T G.656 fiber." ;
    rdfs:subClassOf <http://www.huawei.com/ontology/identity/fiber-type> ;
    prov:wasDerivedFrom "nwi-passive:G656?identity" .

<http://www.huawei.com/ontology/identity/G657A1> a owl:Class,
        owl:NamedIndividual ;
    rdfs:label "G657A1" ;
    rdfs:comment "ITU-T G.657A1 fiber." ;
    rdfs:subClassOf <http://www.huawei.com/ontology/identity/fiber-type> ;
    prov:wasDerivedFrom "nwi-passive:G657A1?identity" .

<http://www.huawei.com/ontology/identity/G657A2> a owl:Class,
        owl:NamedIndividual ;
    rdfs:label "G657A2" ;
    rdfs:comment "ITU-T G.657A2 fiber." ;
    rdfs:subClassOf <http://www.huawei.com/ontology/identity/fiber-type> ;
    prov:wasDerivedFrom "nwi-passive:G657A2?identity" .

<http://www.huawei.com/ontology/identity/G657B> a owl:Class,
        owl:NamedIndividual ;
    rdfs:label "G657B" ;
    rdfs:comment "ITU-T G.657B fiber." ;
    rdfs:subClassOf <http://www.huawei.com/ontology/identity/fiber-type> ;
    prov:wasDerivedFrom "nwi-passive:G657B?identity" .

<http://www.huawei.com/ontology/identity/ODF> a owl:Class,
        owl:NamedIndividual ;
    rdfs:label "ODF" ;
    rdfs:comment "Optical Distribution Frame." ;
    rdfs:subClassOf <http://www.huawei.com/ontology/identity/passive-device-type> ;
    prov:wasDerivedFrom "nwi-passive:ODF?identity" .

<http://www.huawei.com/ontology/identity/WDM> a owl:Class,
        owl:NamedIndividual ;
    rdfs:label "WDM" ;
    rdfs:comment "Wavelength Division Multiplexer." ;
    rdfs:subClassOf <http://www.huawei.com/ontology/identity/passive-device-type> ;
    prov:wasDerivedFrom "nwi-passive:WDM?identity" .

<http://www.huawei.com/ontology/identity/access> a owl:Class,
        owl:NamedIndividual ;
    rdfs:label "access" ;
    rdfs:comment "Access cable." ;
    rdfs:subClassOf <http://www.huawei.com/ontology/identity/cable-role> ;
    prov:wasDerivedFrom "nwi-passive:access?identity" .

<http://www.huawei.com/ontology/identity/accuracy-historic> a owl:Class,
        owl:NamedIndividual ;
    rdfs:label "accuracy-historic" ;
    rdfs:comment """The power data is based on an historic measurement data
for this specific system and usage pattern.""" ;
    rdfs:subClassOf <http://www.huawei.com/ontology/identity/accuracy-estimated> ;
    prov:wasDerivedFrom "eo:accuracy-historic?identity" .

<http://www.huawei.com/ontology/identity/accuracy-learned> a owl:Class,
        owl:NamedIndividual ;
    rdfs:label "accuracy-learned" ;
    rdfs:comment """The power data is based on an machine learning
model prediction.""" ;
    rdfs:subClassOf <http://www.huawei.com/ontology/identity/accuracy-estimated> ;
    prov:wasDerivedFrom "eo:accuracy-learned?identity" .

<http://www.huawei.com/ontology/identity/accuracy-measured-bronze> a owl:Class,
        owl:NamedIndividual ;
    rdfs:label "accuracy-measured-bronze" ;
    rdfs:comment """The power data is a direct, real-time measurement
from a sensor with +/- 30% accuracy for typical values.""" ;
    rdfs:subClassOf <http://www.huawei.com/ontology/identity/accuracy-measured> ;
    prov:wasDerivedFrom "eo:accuracy-measured-bronze?identity" .

<http://www.huawei.com/ontology/identity/accuracy-measured-gold> a owl:Class,
        owl:NamedIndividual ;
    rdfs:label "accuracy-measured-gold" ;
    rdfs:comment """The power data is a direct, real-time measurement
from a sensor with +/- 5% accuracy for typical values.""" ;
    rdfs:subClassOf <http://www.huawei.com/ontology/identity/accuracy-measured> ;
    prov:wasDerivedFrom "eo:accuracy-measured-gold?identity" .

<http://www.huawei.com/ontology/identity/accuracy-measured-ones> a owl:Class,
        owl:NamedIndividual ;
    rdfs:label "accuracy-measured-ones" ;
    rdfs:comment """The power data is a direct, real-time measurement
from a sensor with all non-zero digits valid.""" ;
    rdfs:subClassOf <http://www.huawei.com/ontology/identity/accuracy-measured> ;
    prov:wasDerivedFrom "eo:accuracy-measured-ones?identity" .

<http://www.huawei.com/ontology/identity/accuracy-measured-red> a owl:Class,
        owl:NamedIndividual ;
    rdfs:label "accuracy-measured-red" ;
    rdfs:comment """The power data is a direct, real-time measurement
from a sensor with +/- 2% accuracy for typical values.""" ;
    rdfs:subClassOf <http://www.huawei.com/ontology/identity/accuracy-measured> ;
    prov:wasDerivedFrom "eo:accuracy-measured-red?identity" .

<http://www.huawei.com/ontology/identity/accuracy-measured-silver> a owl:Class,
        owl:NamedIndividual ;
    rdfs:label "accuracy-measured-silver" ;
    rdfs:comment """The power data is a direct, real-time measurement
from a sensor with +/- 10% accuracy for typical values.""" ;
    rdfs:subClassOf <http://www.huawei.com/ontology/identity/accuracy-measured> ;
    prov:wasDerivedFrom "eo:accuracy-measured-silver?identity" .

<http://www.huawei.com/ontology/identity/accuracy-static> a owl:Class,
        owl:NamedIndividual ;
    rdfs:label "accuracy-static" ;
    rdfs:comment """The power data is based on static data, such as
manufacturer specifications, datasheet of typical power values
or nameplate ratings, rather than real-time measurements.""" ;
    rdfs:subClassOf <http://www.huawei.com/ontology/identity/accuracy-estimated> ;
    prov:wasDerivedFrom "eo:accuracy-static?identity" .

<http://www.huawei.com/ontology/identity/accuracy-unavailable> a owl:Class,
        owl:NamedIndividual ;
    rdfs:label "accuracy-unavailable" ;
    rdfs:comment """A power data is not available for some reason, such
as a sensor failure or a component being powered off.""" ;
    rdfs:subClassOf <http://www.huawei.com/ontology/identity/accuracy-unknown> ;
    prov:wasDerivedFrom "eo:accuracy-unavailable?identity" .

<http://www.huawei.com/ontology/identity/active-device> a owl:Class,
        owl:NamedIndividual ;
    rdfs:label "active-device" ;
    rdfs:comment "Active device, e.g. network element." ;
    rdfs:subClassOf <http://www.huawei.com/ontology/identity/connected-device-type> ;
    prov:wasDerivedFrom "nwi-passive:active-device?identity" .

<http://www.huawei.com/ontology/identity/aggregation> a owl:Class,
        owl:NamedIndividual ;
    rdfs:label "aggregation" ;
    rdfs:comment "Aggregation cable." ;
    rdfs:subClassOf <http://www.huawei.com/ontology/identity/cable-role> ;
    prov:wasDerivedFrom "nwi-passive:aggregation?identity" .

<http://www.huawei.com/ontology/identity/backbone> a owl:Class,
        owl:NamedIndividual ;
    rdfs:label "backbone" ;
    rdfs:comment "Backbone cable." ;
    rdfs:subClassOf <http://www.huawei.com/ontology/identity/cable-role> ;
    prov:wasDerivedFrom "nwi-passive:backbone?identity" .

<http://www.huawei.com/ontology/identity/backplane> a owl:Class,
        owl:NamedIndividual ;
    rdfs:label "backplane" ;
    rdfs:comment """This identity is applicable if the hardware class is some sort
of device for aggregating and forwarding networking traffic,
such as a shared backplane in a modular ethernet switch.  Note
that an implementation may model a backplane as a single
physical component, which is actually implemented as multiple
discrete physical components (within a chassis or stack).""" ;
    rdfs:subClassOf <http://www.huawei.com/ontology/identity/hardware-class> ;
    prov:wasDerivedFrom "ianahw:backplane?identity" .

<http://www.huawei.com/ontology/identity/battery> a owl:Class,
        owl:NamedIndividual ;
    rdfs:label "battery" ;
    rdfs:comment """This identity is applicable if the hardware class is some sort
of battery.""" ;
    rdfs:subClassOf <http://www.huawei.com/ontology/identity/hardware-class> ;
    prov:wasDerivedFrom "ianahw:battery?identity" .

<http://www.huawei.com/ontology/identity/branch> a owl:Class,
        owl:NamedIndividual ;
    rdfs:label "branch" ;
    rdfs:comment "Branch cable." ;
    rdfs:subClassOf <http://www.huawei.com/ontology/identity/cable-role> ;
    prov:wasDerivedFrom "nwi-passive:branch?identity" .

<http://www.huawei.com/ontology/identity/chassis> a owl:Class,
        owl:NamedIndividual ;
    rdfs:label "chassis" ;
    rdfs:comment """This identity is applicable if the hardware class is an
overall container for networking equipment.  Any class of
physical component, except a stack, may be contained within a
chassis; a chassis may only be contained within a stack.""" ;
    rdfs:subClassOf <http://www.huawei.com/ontology/identity/hardware-class> ;
    prov:wasDerivedFrom "ianahw:chassis?identity" .

<http://www.huawei.com/ontology/identity/coaxial-cable> a owl:Class,
        owl:NamedIndividual ;
    rdfs:label "coaxial-cable" ;
    rdfs:comment "Coaxial cable." ;
    rdfs:subClassOf <http://www.huawei.com/ontology/identity/electrical-cable> ;
    prov:wasDerivedFrom "nwi-passive:coaxial-cable?identity" .

<http://www.huawei.com/ontology/identity/container> a owl:Class,
        owl:NamedIndividual ;
    rdfs:label "container" ;
    rdfs:comment """This identity is applicable if the hardware class is capable
of containing one or more removable physical entities,
possibly of different types.  For example, each (empty or
full) slot in a chassis will be modeled as a container.  Note
that all removable physical components should be modeled
within a container component, such as field-replaceable
modules, fans, or power supplies.  Note that all known
containers should be modeled by the agent, including empty
containers.""" ;
    rdfs:subClassOf <http://www.huawei.com/ontology/identity/hardware-class> ;
    prov:wasDerivedFrom "ianahw:container?identity" .

<http://www.huawei.com/ontology/identity/cpu> a owl:Class,
        owl:NamedIndividual ;
    rdfs:label "cpu" ;
    rdfs:comment """This identity is applicable if the hardware class is some sort
of central processing unit.""" ;
    rdfs:subClassOf <http://www.huawei.com/ontology/identity/hardware-class> ;
    prov:wasDerivedFrom "ianahw:cpu?identity" .

<http://www.huawei.com/ontology/identity/distribution> a owl:Class,
        owl:NamedIndividual ;
    rdfs:label "distribution" ;
    rdfs:comment "Distribution cable." ;
    rdfs:subClassOf <http://www.huawei.com/ontology/identity/cable-role> ;
    prov:wasDerivedFrom "nwi-passive:distribution?identity" .

<http://www.huawei.com/ontology/identity/energy-object> a owl:Class,
        owl:NamedIndividual ;
    rdfs:label "energy-object" ;
    rdfs:comment """This identity is applicable if the hardware class is some sort
of energy object, i.e., it is a piece of equipment that is
part of or attached to a communications network that is
monitored, it is controlled, or it aids in the management of
another device for Energy Management.""" ;
    rdfs:subClassOf <http://www.huawei.com/ontology/identity/hardware-class> ;
    prov:wasDerivedFrom "ianahw:energy-object?identity" .

<http://www.huawei.com/ontology/identity/fan> a owl:Class,
        owl:NamedIndividual ;
    rdfs:label "fan" ;
    rdfs:comment """This identity is applicable if the hardware class is a fan or
other heat-reduction component.""" ;
    rdfs:subClassOf <http://www.huawei.com/ontology/identity/hardware-class> ;
    prov:wasDerivedFrom "ianahw:fan?identity" .

<http://www.huawei.com/ontology/identity/input-port> a owl:Class,
        owl:NamedIndividual ;
    rdfs:label "input-port" ;
    rdfs:comment "Input port." ;
    rdfs:subClassOf <http://www.huawei.com/ontology/identity/passive-port-type> ;
    prov:wasDerivedFrom "nwi-passive:input-port?identity" .

<http://www.huawei.com/ontology/identity/module> a owl:Class,
        owl:NamedIndividual ;
    rdfs:label "module" ;
    rdfs:comment """This identity is applicable if the hardware class is some sort
of self-contained sub-system.  If a module component is
removable, then it should be modeled within a container
component; otherwise, it should be modeled directly within
another physical component (e.g., a chassis or another
module).""" ;
    rdfs:subClassOf <http://www.huawei.com/ontology/identity/hardware-class> ;
    prov:wasDerivedFrom "ianahw:module?identity" .

<http://www.huawei.com/ontology/identity/multiplier-giga> a owl:Class,
        owl:NamedIndividual ;
    rdfs:label "multiplier-giga" ;
    rdfs:comment """Represents a multiplier of 10^9 (1,000,000,000) associated
with the integer units used to measure the power or energy.""" ;
    prov:wasDerivedFrom "eo:multiplier-giga?identity" .

<http://www.huawei.com/ontology/identity/multiplier-kilo> a owl:Class,
        owl:NamedIndividual ;
    rdfs:label "multiplier-kilo" ;
    rdfs:comment """Represents a multiplier of 10^3 (1,000) associated with the
integer units used to measure the power or energy.""" ;
    prov:wasDerivedFrom "eo:multiplier-kilo?identity" .

<http://www.huawei.com/ontology/identity/multiplier-mega> a owl:Class,
        owl:NamedIndividual ;
    rdfs:label "multiplier-mega" ;
    rdfs:comment """Represents a multiplier of 10^6 (1,000,000) associated with
the integer units used to measure the power or energy.""" ;
    prov:wasDerivedFrom "eo:multiplier-mega?identity" .

<http://www.huawei.com/ontology/identity/multiplier-milli> a owl:Class,
        owl:NamedIndividual ;
    rdfs:label "multiplier-milli" ;
    rdfs:comment """Represents a multiplier of 10^-3 (0.001) associated with the
integer units used to measure the power or energy.""" ;
    prov:wasDerivedFrom "eo:multiplier-milli?identity" .

<http://www.huawei.com/ontology/identity/multiplier-none> a owl:Class,
        owl:NamedIndividual ;
    rdfs:label "multiplier-none" ;
    rdfs:comment """Represents a multiplier of 10^0 (1) associated with
the integer units used to measure the power or energy.""" ;
    prov:wasDerivedFrom "eo:multiplier-none?identity" .

<http://www.huawei.com/ontology/identity/ne-physical> a owl:Class,
        owl:NamedIndividual ;
    rdfs:label "ne-physical" ;
    rdfs:comment "A physical network element (NE). " ;
    rdfs:subClassOf <http://www.huawei.com/ontology/identity/ne-type> ;
    prov:wasDerivedFrom "nwi:ne-physical?identity" .

<http://www.huawei.com/ontology/identity/non-hardware-component-class> a owl:Class,
        owl:NamedIndividual ;
    rdfs:label "non-hardware-component-class" ;
    rdfs:comment """Base identity for non hardware components (e.g., software
components) in a managed device.""" ;
    prov:wasDerivedFrom "nwi:non-hardware-component-class?identity" .

<http://www.huawei.com/ontology/identity/optical-fiber> a owl:Class,
        owl:NamedIndividual ;
    rdfs:label "optical-fiber" ;
    rdfs:comment "Fiber optic cable." ;
    rdfs:subClassOf <http://www.huawei.com/ontology/identity/cable-type> ;
    prov:wasDerivedFrom "nwi-passive:optical-fiber?identity" .

<http://www.huawei.com/ontology/identity/other> a owl:Class,
        owl:NamedIndividual ;
    rdfs:label "other" ;
    rdfs:comment "Other type of fiber." ;
    rdfs:subClassOf <http://www.huawei.com/ontology/identity/fiber-type> ;
    prov:wasDerivedFrom "nwi-passive:other?identity" .

<http://www.huawei.com/ontology/identity/output-port> a owl:Class,
        owl:NamedIndividual ;
    rdfs:label "output-port" ;
    rdfs:comment "Output port." ;
    rdfs:subClassOf <http://www.huawei.com/ontology/identity/passive-port-type> ;
    prov:wasDerivedFrom "nwi-passive:output-port?identity" .

<http://www.huawei.com/ontology/identity/p2mp-port> a owl:Class,
        owl:NamedIndividual ;
    rdfs:label "p2mp-port" ;
    rdfs:comment "Input port." ;
    rdfs:subClassOf <http://www.huawei.com/ontology/identity/passive-port-type> ;
    prov:wasDerivedFrom "nwi-passive:p2mp-port?identity" .

<http://www.huawei.com/ontology/identity/passive-device> a owl:Class,
        owl:NamedIndividual ;
    rdfs:label "passive-device" ;
    rdfs:comment "Passive/unmanaged device." ;
    rdfs:subClassOf <http://www.huawei.com/ontology/identity/connected-device-type> ;
    prov:wasDerivedFrom "nwi-passive:passive-device?identity" .

<http://www.huawei.com/ontology/identity/port> a owl:Class,
        owl:NamedIndividual ;
    rdfs:label "port" ;
    rdfs:comment """This identity is applicable if the hardware class is some sort
of networking port capable of receiving and/or transmitting
networking traffic.""" ;
    rdfs:subClassOf <http://www.huawei.com/ontology/identity/hardware-class> ;
    prov:wasDerivedFrom "ianahw:port?identity" .

<http://www.huawei.com/ontology/identity/power-state> a owl:Class,
        owl:NamedIndividual ;
    rdfs:label "power-state" ;
    rdfs:comment """Base identity for all possible power states. This identity
serves as the root for a hierarchy of power states, allowing
for extensibility while maintaining alignment with the IANA
Power State Set Registry.""" ;
    prov:wasDerivedFrom "eo:power-state?identity" .

<http://www.huawei.com/ontology/identity/power-supply> a owl:Class,
        owl:NamedIndividual ;
    rdfs:label "power-supply" ;
    rdfs:comment """This identity is applicable if the hardware class is a
power-supplying component.""" ;
    rdfs:subClassOf <http://www.huawei.com/ontology/identity/hardware-class> ;
    prov:wasDerivedFrom "ianahw:power-supply?identity" .

<http://www.huawei.com/ontology/identity/sensor> a owl:Class,
        owl:NamedIndividual ;
    rdfs:label "sensor" ;
    rdfs:comment """This identity is applicable if the hardware class is some sort
of sensor, such as a temperature sensor within a router
chassis.""" ;
    rdfs:subClassOf <http://www.huawei.com/ontology/identity/hardware-class> ;
    prov:wasDerivedFrom "ianahw:sensor?identity" .

<http://www.huawei.com/ontology/identity/service-port> a owl:Class,
        owl:NamedIndividual ;
    rdfs:label "service-port" ;
    rdfs:comment "Service port." ;
    rdfs:subClassOf <http://www.huawei.com/ontology/identity/passive-port-type> ;
    prov:wasDerivedFrom "nwi-passive:service-port?identity" .

<http://www.huawei.com/ontology/identity/stack> a owl:Class,
        owl:NamedIndividual ;
    rdfs:label "stack" ;
    rdfs:comment """This identity is applicable if the hardware class is some sort
of super-container (possibly virtual) intended to group
together multiple chassis entities.  A stack may be realized
by a virtual cable, a real interconnect cable attached to
multiple chassis, or multiple interconnect cables.  A stack
should not be modeled within any other physical components,
but a stack may be contained within another stack.  Only
chassis components should be contained within a stack.""" ;
    rdfs:subClassOf <http://www.huawei.com/ontology/identity/hardware-class> ;
    prov:wasDerivedFrom "ianahw:stack?identity" .

<http://www.huawei.com/ontology/identity/storage-drive> a owl:Class,
        owl:NamedIndividual ;
    rdfs:label "storage-drive" ;
    rdfs:comment """This identity is applicable if the hardware class is some sort
of component with data storage capability as its main
functionality, e.g., hard disk drive (HDD), solid-state device
(SSD), solid-state hybrid drive (SSHD), object storage device
(OSD), or other.""" ;
    rdfs:subClassOf <http://www.huawei.com/ontology/identity/hardware-class> ;
    prov:wasDerivedFrom "ianahw:storage-drive?identity" .

<http://www.huawei.com/ontology/identity/trunk> a owl:Class,
        owl:NamedIndividual ;
    rdfs:label "trunk" ;
    rdfs:comment "Trunk cable." ;
    rdfs:subClassOf <http://www.huawei.com/ontology/identity/cable-role> ;
    prov:wasDerivedFrom "nwi-passive:trunk?identity" .

<http://www.huawei.com/ontology/identity/unknown> a owl:Class,
        owl:NamedIndividual ;
    rdfs:label "unknown" ;
    rdfs:comment """This identity is applicable if the hardware class is unknown
to the server.""" ;
    rdfs:subClassOf <http://www.huawei.com/ontology/identity/hardware-class> ;
    prov:wasDerivedFrom "ianahw:unknown?identity" .

<http://www.huawei.com/ontology/ietf-hardware/hardware/component/alias> a owl:DatatypeProperty ;
    rdfs:label "alias" ;
    rdfs:comment """An 'alias' name for the component, as specified by a
network manager, that provides a non-volatile 'handle' for
the component.

If no configured value exists, the server MAY set the
value of this node to a locally unique value in the
operational state.

A server implementation MAY map this leaf to the
entPhysicalAlias MIB object.  Such an implementation needs
to use some mechanism to handle the differences in size
and characters allowed between this leaf and
entPhysicalAlias.  The definition of such a mechanism is
outside the scope of this document.""" ;
    rdfs:domain <http://www.huawei.com/ontology/ietf-hardware/hardware/component> ;
    rdfs:range xsd:string ;
    prov:wasDerivedFrom "hw:hardware?container/hw:component?list/hw:alias?leaf" .

<http://www.huawei.com/ontology/ietf-hardware/hardware/component/asset-id> a owl:DatatypeProperty ;
    rdfs:label "asset-id" ;
    rdfs:comment """This node is a user-assigned asset tracking identifier for
the component.

A server implementation MAY map this leaf to the
entPhysicalAssetID MIB object.  Such an implementation
needs to use some mechanism to handle the differences in
size and characters allowed between this leaf and
entPhysicalAssetID.  The definition of such a mechanism is
outside the scope of this document.""" ;
    rdfs:domain <http://www.huawei.com/ontology/ietf-hardware/hardware/component> ;
    rdfs:range xsd:string ;
    prov:wasDerivedFrom "hw:hardware?container/hw:component?list/hw:asset-id?leaf" .

<http://www.huawei.com/ontology/ietf-hardware/hardware/component/class> a owl:ObjectProperty ;
    rdfs:label "class" ;
    rdfs:comment """An indication of the general hardware type of the
component.""" ;
    rdfs:domain <http://www.huawei.com/ontology/ietf-hardware/hardware/component> ;
    rdfs:range <http://www.huawei.com/ontology/identity/hardware-class> ;
    owl:minCardinality 0 ;
    prov:wasDerivedFrom "hw:hardware?container/hw:component?list/hw:class?leaf" .

<http://www.huawei.com/ontology/ietf-hardware/hardware/component/contains-child> a owl:ObjectProperty ;
    ex:xpathPath "../../component/name" ;
    rdfs:comment "The name of the contained component." ;
    rdfs:domain <http://www.huawei.com/ontology/ietf-hardware/hardware/component> ;
    rdfs:range <http://www.huawei.com/ontology/ietf-hardware/hardware/component> ;
    owl:minCardinality 0 ;
    prov:wasDerivedFrom "hw:hardware?container/hw:component?list/hw:contains-child?leaf-list" .

<http://www.huawei.com/ontology/ietf-hardware/hardware/component/description> a owl:DatatypeProperty ;
    rdfs:label "description" ;
    rdfs:comment """A textual description of the component.  This node should
contain a string that identifies the manufacturer's name
for the component and should be set to a distinct value
for each version or model of the component.""" ;
    rdfs:domain <http://www.huawei.com/ontology/ietf-hardware/hardware/component> ;
    rdfs:range xsd:string ;
    prov:wasDerivedFrom "hw:hardware?container/hw:component?list/hw:description?leaf" .

<http://www.huawei.com/ontology/ietf-hardware/hardware/component/firmware-rev> a owl:DatatypeProperty ;
    rdfs:label "firmware-rev" ;
    rdfs:comment """The vendor-specific firmware revision string for the
component.""" ;
    rdfs:domain <http://www.huawei.com/ontology/ietf-hardware/hardware/component> ;
    rdfs:range xsd:string ;
    prov:wasDerivedFrom "hw:hardware?container/hw:component?list/hw:firmware-rev?leaf" .

<http://www.huawei.com/ontology/ietf-hardware/hardware/component/hardware-rev> a owl:DatatypeProperty ;
    rdfs:label "hardware-rev" ;
    rdfs:comment """The vendor-specific hardware revision string for the
component.  The preferred value is the hardware revision
identifier actually printed on the component itself (if
present).""" ;
    rdfs:domain <http://www.huawei.com/ontology/ietf-hardware/hardware/component> ;
    rdfs:range xsd:string ;
    prov:wasDerivedFrom "hw:hardware?container/hw:component?list/hw:hardware-rev?leaf" .

<http://www.huawei.com/ontology/ietf-hardware/hardware/component/hasSensorData> a owl:ObjectProperty ;
    rdfs:label "hasSensorData" ;
    rdfs:comment "Containment relation (parent --> child)." ;
    rdfs:domain <http://www.huawei.com/ontology/ietf-hardware/hardware/component> ;
    rdfs:range <http://www.huawei.com/ontology/ietf-hardware/hardware/component/sensor-data> ;
    owl:minCardinality 0 ;
    prov:wasDerivedFrom "hw:hardware?container/hw:component?list/hasSensorData" .

<http://www.huawei.com/ontology/ietf-hardware/hardware/component/hasState> a owl:ObjectProperty ;
    rdfs:label "hasState" ;
    rdfs:comment "Containment relation (parent --> child)." ;
    rdfs:domain <http://www.huawei.com/ontology/ietf-hardware/hardware/component> ;
    rdfs:range <http://www.huawei.com/ontology/ietf-hardware/hardware/component/state> ;
    owl:minCardinality 0 ;
    prov:wasDerivedFrom "hw:hardware?container/hw:component?list/hasState" .

<http://www.huawei.com/ontology/ietf-hardware/hardware/component/is-fru> a owl:DatatypeProperty ;
    rdfs:label "is-fru" ;
    rdfs:comment """This node indicates whether or not this component is
considered a 'field-replaceable unit' by the vendor.  If
this node contains the value 'true', then this component
identifies a field-replaceable unit.  For all components
that are permanently contained within a field-replaceable
unit, the value 'false' should be returned for this
node.""" ;
    rdfs:domain <http://www.huawei.com/ontology/ietf-hardware/hardware/component> ;
    rdfs:range xsd:boolean ;
    prov:wasDerivedFrom "hw:hardware?container/hw:component?list/hw:is-fru?leaf" .

<http://www.huawei.com/ontology/ietf-hardware/hardware/component/mfg-date> a owl:DatatypeProperty ;
    rdfs:label "mfg-date" ;
    rdfs:comment "The date of manufacturing of the managed component." ;
    rdfs:domain <http://www.huawei.com/ontology/ietf-hardware/hardware/component> ;
    rdfs:range xsd:dateTime ;
    prov:wasDerivedFrom "hw:hardware?container/hw:component?list/hw:mfg-date?leaf" .

<http://www.huawei.com/ontology/ietf-hardware/hardware/component/mfg-name> a owl:DatatypeProperty ;
    rdfs:label "mfg-name" ;
    rdfs:comment """The name of the manufacturer of this physical component.
The preferred value is the manufacturer name string
actually printed on the component itself (if present).

Note that comparisons between instances of the
'model-name', 'firmware-rev', 'software-rev', and
'serial-num' nodes are only meaningful amongst components
with the same value of 'mfg-name'.

If the manufacturer name string associated with the
physical component is unknown to the server, then this
node is not instantiated.""" ;
    rdfs:domain <http://www.huawei.com/ontology/ietf-hardware/hardware/component> ;
    rdfs:range xsd:string ;
    prov:wasDerivedFrom "hw:hardware?container/hw:component?list/hw:mfg-name?leaf" .

<http://www.huawei.com/ontology/ietf-hardware/hardware/component/model-name> a owl:DatatypeProperty ;
    rdfs:label "model-name" ;
    rdfs:comment """The vendor-specific model name identifier string
associated with this physical component.  The preferred
value is the customer-visible part number, which may be
printed on the component itself.

If the model name string associated with the physical
component is unknown to the server, then this node is not
instantiated.""" ;
    rdfs:domain <http://www.huawei.com/ontology/ietf-hardware/hardware/component> ;
    rdfs:range xsd:string ;
    prov:wasDerivedFrom "hw:hardware?container/hw:component?list/hw:model-name?leaf" .

<http://www.huawei.com/ontology/ietf-hardware/hardware/component/name> a owl:DatatypeProperty ;
    rdfs:label "name" ;
    rdfs:comment """The name assigned to this component.

This name is not required to be the same as
entPhysicalName.""" ;
    rdfs:domain <http://www.huawei.com/ontology/ietf-hardware/hardware/component> ;
    rdfs:range xsd:string ;
    prov:wasDerivedFrom "hw:hardware?container/hw:component?list/hw:name?leaf" .

<http://www.huawei.com/ontology/ietf-hardware/hardware/component/parent> a owl:ObjectProperty ;
    ex:xpathPath "../../component/name" ;
    rdfs:comment """The name of the component that physically contains this
component.

If this leaf is not instantiated, it indicates that this
component is not contained in any other component.

In the event that a physical component is contained by
more than one physical component (e.g., double-wide
modules), this node contains the name of one of these
components.  An implementation MUST use the same name
every time this node is instantiated.""" ;
    rdfs:domain <http://www.huawei.com/ontology/ietf-hardware/hardware/component> ;
    rdfs:range <http://www.huawei.com/ontology/ietf-hardware/hardware/component> ;
    owl:minCardinality 0 ;
    prov:wasDerivedFrom "hw:hardware?container/hw:component?list/hw:parent?leaf" .

<http://www.huawei.com/ontology/ietf-hardware/hardware/component/parent-rel-pos> a owl:DatatypeProperty ;
    rdfs:label "parent-rel-pos" ;
    rdfs:comment """An indication of the relative position of this child
component among all its sibling components.  Sibling
components are defined as components that:

  o share the same value of the 'parent' node and

  o share a common base identity for the 'class' node.

Note that the last rule gives implementations flexibility
in how components are numbered.  For example, some
implementations might have a single number series for all
components derived from 'ianahw:port', while some others
might have different number series for different
components with identities derived from 'ianahw:port' (for
example, one for registered jack 45 (RJ45) and one for
small form-factor pluggable (SFP)).""" ;
    rdfs:domain <http://www.huawei.com/ontology/ietf-hardware/hardware/component> ;
    rdfs:range xsd:int ;
    prov:wasDerivedFrom "hw:hardware?container/hw:component?list/hw:parent-rel-pos?leaf" .

<http://www.huawei.com/ontology/ietf-hardware/hardware/component/physical-index> a owl:DatatypeProperty ;
    rdfs:label "physical-index" ;
    rdfs:comment """The entPhysicalIndex for the entPhysicalEntry represented
by this list entry.""" ;
    rdfs:domain <http://www.huawei.com/ontology/ietf-hardware/hardware/component> ;
    rdfs:range xsd:int ;
    prov:wasDerivedFrom "hw:hardware?container/hw:component?list/hw:physical-index?leaf" .

<http://www.huawei.com/ontology/ietf-hardware/hardware/component/sensor-data/oper-status> a owl:DatatypeProperty ;
    rdfs:label "oper-status" ;
    rdfs:comment "The operational status of the sensor." ;
    rdfs:domain <http://www.huawei.com/ontology/ietf-hardware/hardware/component/sensor-data> ;
    rdfs:range rdfs:Literal ;
    prov:wasDerivedFrom "hw:hardware?container/hw:component?list/hw:sensor-data?container/hw:oper-status?leaf" .

<http://www.huawei.com/ontology/ietf-hardware/hardware/component/sensor-data/units-display> a owl:DatatypeProperty ;
    rdfs:label "units-display" ;
    rdfs:comment """A textual description of the data units that should be
used in the display of the sensor value.""" ;
    rdfs:domain <http://www.huawei.com/ontology/ietf-hardware/hardware/component/sensor-data> ;
    rdfs:range xsd:string ;
    prov:wasDerivedFrom "hw:hardware?container/hw:component?list/hw:sensor-data?container/hw:units-display?leaf" .

<http://www.huawei.com/ontology/ietf-hardware/hardware/component/sensor-data/value> a owl:DatatypeProperty ;
    rdfs:label "value" ;
    rdfs:comment """The most recent measurement obtained by the server
for this sensor.

A client that periodically fetches this node should also
fetch the nodes 'value-type', 'value-scale', and
'value-precision', since they may change when the value
is changed.""" ;
    rdfs:domain <http://www.huawei.com/ontology/ietf-hardware/hardware/component/sensor-data> ;
    rdfs:range xsd:int ;
    prov:wasDerivedFrom "hw:hardware?container/hw:component?list/hw:sensor-data?container/hw:value?leaf" .

<http://www.huawei.com/ontology/ietf-hardware/hardware/component/sensor-data/value-precision> a owl:DatatypeProperty ;
    rdfs:label "value-precision" ;
    rdfs:comment """The number of decimal places of precision
associated with the sensor value""" ;
    rdfs:domain <http://www.huawei.com/ontology/ietf-hardware/hardware/component/sensor-data> ;
    rdfs:range xsd:byte ;
    prov:wasDerivedFrom "hw:hardware?container/hw:component?list/hw:sensor-data?container/hw:value-precision?leaf" .

<http://www.huawei.com/ontology/ietf-hardware/hardware/component/sensor-data/value-scale> a owl:DatatypeProperty ;
    rdfs:label "value-scale" ;
    rdfs:comment """The (power of 10) scaling factor associated
with the sensor value""" ;
    rdfs:domain <http://www.huawei.com/ontology/ietf-hardware/hardware/component/sensor-data> ;
    rdfs:range rdfs:Literal ;
    prov:wasDerivedFrom "hw:hardware?container/hw:component?list/hw:sensor-data?container/hw:value-scale?leaf" .

<http://www.huawei.com/ontology/ietf-hardware/hardware/component/sensor-data/value-timestamp> a owl:DatatypeProperty ;
    rdfs:label "value-timestamp" ;
    rdfs:comment """The time the status and/or value of this sensor was last
obtained by the server.""" ;
    rdfs:domain <http://www.huawei.com/ontology/ietf-hardware/hardware/component/sensor-data> ;
    rdfs:range xsd:dateTime ;
    prov:wasDerivedFrom "hw:hardware?container/hw:component?list/hw:sensor-data?container/hw:value-timestamp?leaf" .

<http://www.huawei.com/ontology/ietf-hardware/hardware/component/sensor-data/value-type> a owl:DatatypeProperty ;
    rdfs:label "value-type" ;
    rdfs:comment """The type of data units associated with the
sensor value""" ;
    rdfs:domain <http://www.huawei.com/ontology/ietf-hardware/hardware/component/sensor-data> ;
    rdfs:range rdfs:Literal ;
    prov:wasDerivedFrom "hw:hardware?container/hw:component?list/hw:sensor-data?container/hw:value-type?leaf" .

<http://www.huawei.com/ontology/ietf-hardware/hardware/component/sensor-data/value-update-rate> a owl:DatatypeProperty ;
    rdfs:label "value-update-rate" ;
    rdfs:comment """An indication of the frequency that the server updates
the associated 'value' node, represented in
milliseconds.  The value zero indicates:

 - the sensor value is updated on demand (e.g.,
   when polled by the server for a get-request),

 - the sensor value is updated when the sensor
   value changes (event-driven), or

 - the server does not know the update rate.""" ;
    rdfs:domain <http://www.huawei.com/ontology/ietf-hardware/hardware/component/sensor-data> ;
    rdfs:range xsd:unsignedInt ;
    prov:wasDerivedFrom "hw:hardware?container/hw:component?list/hw:sensor-data?container/hw:value-update-rate?leaf" .

<http://www.huawei.com/ontology/ietf-hardware/hardware/component/serial-num> a owl:DatatypeProperty ;
    rdfs:label "serial-num" ;
    rdfs:comment """The vendor-specific serial number string for the
component.  The preferred value is the serial number
string actually printed on the component itself (if
present).""" ;
    rdfs:domain <http://www.huawei.com/ontology/ietf-hardware/hardware/component> ;
    rdfs:range xsd:string ;
    prov:wasDerivedFrom "hw:hardware?container/hw:component?list/hw:serial-num?leaf" .

<http://www.huawei.com/ontology/ietf-hardware/hardware/component/software-rev> a owl:DatatypeProperty ;
    rdfs:label "software-rev" ;
    rdfs:comment """The vendor-specific software revision string for the
component.""" ;
    rdfs:domain <http://www.huawei.com/ontology/ietf-hardware/hardware/component> ;
    rdfs:range xsd:string ;
    prov:wasDerivedFrom "hw:hardware?container/hw:component?list/hw:software-rev?leaf" .

<http://www.huawei.com/ontology/ietf-hardware/hardware/component/state/admin-state> a owl:DatatypeProperty ;
    rdfs:label "admin-state" ;
    rdfs:comment """The administrative state for this component.

This node refers to a component's administrative
permission to service both other components within its
containment hierarchy as well other users of its
services defined by means outside the scope of this
module.

Some components exhibit only a subset of the remaining
administrative state values.  Some components cannot be
locked; hence, this node exhibits only the 'unlocked'
state.  Other components cannot be shut down gracefully;
hence, this node does not exhibit the 'shutting-down'
state.""" ;
    rdfs:domain <http://www.huawei.com/ontology/ietf-hardware/hardware/component/state> ;
    rdfs:range rdfs:Literal ;
    prov:wasDerivedFrom "hw:hardware?container/hw:component?list/hw:state?container/hw:admin-state?leaf" .

<http://www.huawei.com/ontology/ietf-hardware/hardware/component/state/alarm-state> a owl:DatatypeProperty ;
    rdfs:label "alarm-state" ;
    rdfs:comment """The alarm state for this component.  It does not
include the alarms raised on child components within its
containment hierarchy.""" ;
    rdfs:domain <http://www.huawei.com/ontology/ietf-hardware/hardware/component/state> ;
    rdfs:range rdfs:Literal ;
    prov:wasDerivedFrom "hw:hardware?container/hw:component?list/hw:state?container/hw:alarm-state?leaf" .

<http://www.huawei.com/ontology/ietf-hardware/hardware/component/state/oper-state> a owl:DatatypeProperty ;
    rdfs:label "oper-state" ;
    rdfs:comment """The operational state for this component.

Note that this node does not follow the administrative
state.  An administrative state of 'down' does not
predict an operational state of 'disabled'.

Note that some implementations may not be able to
accurately report oper-state while the admin-state node
has a value other than 'unlocked'.  In these cases, this
node MUST have a value of 'unknown'.""" ;
    rdfs:domain <http://www.huawei.com/ontology/ietf-hardware/hardware/component/state> ;
    rdfs:range rdfs:Literal ;
    prov:wasDerivedFrom "hw:hardware?container/hw:component?list/hw:state?container/hw:oper-state?leaf" .

<http://www.huawei.com/ontology/ietf-hardware/hardware/component/state/standby-state> a owl:DatatypeProperty ;
    rdfs:label "standby-state" ;
    rdfs:comment """The standby state for this component.

Some components will exhibit only a subset of the
remaining standby state values.  If this component
cannot operate in a standby role, the value of this node
will always be 'providing-service'.""" ;
    rdfs:domain <http://www.huawei.com/ontology/ietf-hardware/hardware/component/state> ;
    rdfs:range rdfs:Literal ;
    prov:wasDerivedFrom "hw:hardware?container/hw:component?list/hw:state?container/hw:standby-state?leaf" .

<http://www.huawei.com/ontology/ietf-hardware/hardware/component/state/state-last-changed> a owl:DatatypeProperty ;
    rdfs:label "state-last-changed" ;
    rdfs:comment """The date and time when the value of any of the
admin-state, oper-state, usage-state, alarm-state, or
standby-state changed for this component.

If there has been no change since the last
re-initialization of the local system, this node
contains the date and time of local system
initialization.  If there has been no change since the
component was added to the local system, this node
contains the date and time of the insertion.""" ;
    rdfs:domain <http://www.huawei.com/ontology/ietf-hardware/hardware/component/state> ;
    rdfs:range xsd:dateTime ;
    prov:wasDerivedFrom "hw:hardware?container/hw:component?list/hw:state?container/hw:state-last-changed?leaf" .

<http://www.huawei.com/ontology/ietf-hardware/hardware/component/state/usage-state> a owl:DatatypeProperty ;
    rdfs:label "usage-state" ;
    rdfs:comment """The usage state for this component.

This node refers to a component's ability to service
more components in a containment hierarchy.

Some components will exhibit only a subset of the usage
state values.  Components that are unable to ever
service any components within a containment hierarchy
will always have a usage state of 'busy'.  In some
cases, a component will be able to support only one
other component within its containment hierarchy and
will therefore only exhibit values of 'idle' and
'busy'.""" ;
    rdfs:domain <http://www.huawei.com/ontology/ietf-hardware/hardware/component/state> ;
    rdfs:range rdfs:Literal ;
    prov:wasDerivedFrom "hw:hardware?container/hw:component?list/hw:state?container/hw:usage-state?leaf" .

<http://www.huawei.com/ontology/ietf-hardware/hardware/component/uri> a owl:DatatypeProperty ;
    rdfs:label "uri" ;
    rdfs:comment """This node contains identification information about the
component.""" ;
    rdfs:domain <http://www.huawei.com/ontology/ietf-hardware/hardware/component> ;
    rdfs:range xsd:string ;
    prov:wasDerivedFrom "hw:hardware?container/hw:component?list/hw:uri?leaf-list" .

<http://www.huawei.com/ontology/ietf-hardware/hardware/component/uuid> a owl:DatatypeProperty ;
    rdfs:label "uuid" ;
    rdfs:comment "A Universally Unique Identifier of the component." ;
    rdfs:domain <http://www.huawei.com/ontology/ietf-hardware/hardware/component> ;
    rdfs:range xsd:string ;
    prov:wasDerivedFrom "hw:hardware?container/hw:component?list/hw:uuid?leaf" .

<http://www.huawei.com/ontology/ietf-hardware/hardware/hasComponent> a owl:ObjectProperty ;
    rdfs:label "hasComponent" ;
    rdfs:comment "Containment relation (parent --> child)." ;
    rdfs:domain <http://www.huawei.com/ontology/ietf-hardware/hardware> ;
    rdfs:range <http://www.huawei.com/ontology/ietf-hardware/hardware/component> ;
    owl:minCardinality 0 ;
    prov:wasDerivedFrom "hw:hardware?container/hasComponent" .

<http://www.huawei.com/ontology/ietf-hardware/hardware/last-change> a owl:DatatypeProperty ;
    rdfs:label "last-change" ;
    rdfs:comment """The time the '/hardware/component' list changed in the
operational state.""" ;
    rdfs:domain <http://www.huawei.com/ontology/ietf-hardware/hardware> ;
    rdfs:range xsd:dateTime ;
    prov:wasDerivedFrom "hw:hardware?container/hw:last-change?leaf" .

<http://www.huawei.com/ontology/ietf-network-inventory-txt/network-inventory/hasNetworkElements> a owl:ObjectProperty ;
    rdfs:label "hasNetworkElements" ;
    rdfs:comment "Containment relation (parent --> child)." ;
    rdfs:domain <http://www.huawei.com/ontology/ietf-network-inventory-txt/network-inventory> ;
    rdfs:range <http://www.huawei.com/ontology/ietf-network-inventory-txt/network-inventory/network-elements> ;
    owl:minCardinality 0 ;
    prov:wasDerivedFrom "nwi:network-inventory?container/hasNetworkElements" .

<http://www.huawei.com/ontology/ietf-network-inventory-txt/network-inventory/network-elements/hasNetworkElement> a owl:ObjectProperty ;
    rdfs:label "hasNetworkElement" ;
    rdfs:comment "Containment relation (parent --> child)." ;
    rdfs:domain <http://www.huawei.com/ontology/ietf-network-inventory-txt/network-inventory/network-elements> ;
    rdfs:range <http://www.huawei.com/ontology/ietf-network-inventory-txt/network-inventory/network-elements/network-element> ;
    owl:minCardinality 0 ;
    prov:wasDerivedFrom "nwi:network-inventory?container/nwi:network-elements?container/hasNetworkElement" .

<http://www.huawei.com/ontology/ietf-network-inventory-txt/network-inventory/network-elements/network-element/components/component/is-main> a owl:DatatypeProperty ;
    rdfs:label "is-main" ;
    rdfs:comment "Conditional: exists when derived-from-or-self(../nwi:class, 'ianahw:chassis')",
        """This node indicates whether the chassis is taking or
not the 'main' role.

This node is applicable only to scenarios where
there are chassis components which can take the
'main' role (e.g., multi-chassis network elements),
otherwise it is omitted.""" ;
    rdfs:domain <http://www.huawei.com/ontology/ietf-network-inventory-txt/network-inventory/network-elements/network-element/components/component> ;
    rdfs:range xsd:boolean ;
    prov:wasDerivedFrom "nwi:network-inventory?container/nwi:network-elements?container/nwi:network-element?list/nwi:components?container/nwi:component?list/nwi:is-main?leaf" ;
    sh:deactivated "derived-from-or-self(../nwi:class, 'ianahw:chassis')" .

<http://www.huawei.com/ontology/ietf-network-inventory-txt/network-inventory/network-elements/network-element/components/component/parent> a owl:ObjectProperty ;
    ex:xpathPath "../../component/component-id" ;
    rdfs:comment """The identifiers of all the components that
physically contain this component.

If this list is empty, this component is not
contained in any other component but it is contained
in the network-element.""" ;
    rdfs:domain <http://www.huawei.com/ontology/ietf-network-inventory-txt/network-inventory/network-elements/network-element/components/component> ;
    rdfs:range <http://www.huawei.com/ontology/ietf-network-inventory-txt/network-inventory/network-elements/network-element/components/component> ;
    owl:minCardinality 0 ;
    prov:wasDerivedFrom "nwi:network-inventory?container/nwi:network-elements?container/nwi:network-element?list/nwi:components?container/nwi:component?list/nwi:parent?leaf-list" .

<http://www.huawei.com/ontology/ietf-network-inventory-txt/network-inventory/network-elements/network-element/components/component/parent-rel-pos> a owl:DatatypeProperty ;
    rdfs:label "parent-rel-pos" ;
    rdfs:comment "Conditional: exists when count(../parent) < 2",
        """The relative position with respect to the parent
component among all the sibling components.""" ;
    rdfs:domain <http://www.huawei.com/ontology/ietf-network-inventory-txt/network-inventory/network-elements/network-element/components/component> ;
    rdfs:range xsd:int ;
    prov:wasDerivedFrom "nwi:network-inventory?container/nwi:network-elements?container/nwi:network-element?list/nwi:components?container/nwi:component?list/nwi:parent-rel-pos?leaf" ;
    sh:deactivated "count(../parent) < 2" .

<http://www.huawei.com/ontology/ietf-network-inventory-txt/network-inventory/network-elements/network-element/components/hasComponent> a owl:ObjectProperty ;
    rdfs:label "hasComponent" ;
    rdfs:comment "Containment relation (parent --> child)." ;
    rdfs:domain <http://www.huawei.com/ontology/ietf-network-inventory-txt/network-inventory/network-elements/network-element/components> ;
    rdfs:range <http://www.huawei.com/ontology/ietf-network-inventory-txt/network-inventory/network-elements/network-element/components/component> ;
    owl:minCardinality 0 ;
    prov:wasDerivedFrom "nwi:network-inventory?container/nwi:network-elements?container/nwi:network-element?list/nwi:components?container/hasComponent" .

<http://www.huawei.com/ontology/ietf-network-inventory-txt/network-inventory/network-elements/network-element/hasComponents> a owl:ObjectProperty ;
    rdfs:label "hasComponents" ;
    rdfs:comment "Containment relation (parent --> child)." ;
    rdfs:domain <http://www.huawei.com/ontology/ietf-network-inventory-txt/network-inventory/network-elements/network-element> ;
    rdfs:range <http://www.huawei.com/ontology/ietf-network-inventory-txt/network-inventory/network-elements/network-element/components> ;
    owl:minCardinality 0 ;
    prov:wasDerivedFrom "nwi:network-inventory?container/nwi:network-elements?container/nwi:network-element?list/hasComponents" .

<http://www.huawei.com/ontology/ietf-network-inventory-txt/network-inventory/network-elements/network-element/ne-id> a owl:DatatypeProperty ;
    rdfs:label "ne-id" ;
    rdfs:comment """An identifier that uniquely identifies the NE in
a network.""" ;
    rdfs:domain <http://www.huawei.com/ontology/ietf-network-inventory-txt/network-inventory/network-elements/network-element> ;
    rdfs:range xsd:string ;
    prov:wasDerivedFrom "nwi:network-inventory?container/nwi:network-elements?container/nwi:network-element?list/nwi:ne-id?leaf" .

<http://www.huawei.com/ontology/ietf-network-inventory-txt/network-inventory/network-elements/network-element/ne-type> a owl:ObjectProperty ;
    rdfs:label "ne-type" ;
    rdfs:comment "The network element type." ;
    rdfs:domain <http://www.huawei.com/ontology/ietf-network-inventory-txt/network-inventory/network-elements/network-element> ;
    rdfs:range <http://www.huawei.com/ontology/identity/ne-type> ;
    owl:minCardinality 0 ;
    prov:wasDerivedFrom "nwi:network-inventory?container/nwi:network-elements?container/nwi:network-element?list/nwi:ne-type?leaf" .

<http://www.huawei.com/ontology/ietf-network-inventory-txt/network-inventory/network-elements/network-element/product-rev> a owl:DatatypeProperty ;
    rdfs:label "product-rev" ;
    rdfs:comment """The vendor-specific product revision string for the
network-element.""" ;
    rdfs:domain <http://www.huawei.com/ontology/ietf-network-inventory-txt/network-inventory/network-elements/network-element> ;
    rdfs:range xsd:string ;
    prov:wasDerivedFrom "nwi:network-inventory?container/nwi:network-elements?container/nwi:network-element?list/nwi:product-rev?leaf" .

<http://www.huawei.com/ontology/ietf-network/networks/network/hasLink> a owl:ObjectProperty ;
    rdfs:label "hasLink" ;
    rdfs:comment "Containment relation (parent --> child)." ;
    rdfs:domain <http://www.huawei.com/ontology/ietf-network/networks/network> ;
    rdfs:range <http://www.huawei.com/ontology/ietf-network/networks/network/link> ;
    owl:minCardinality 0 .

<http://www.huawei.com/ontology/ietf-network/networks/network/hasNode> a owl:ObjectProperty ;
    rdfs:label "hasNode" ;
    rdfs:comment "Containment relation (parent --> child)." ;
    rdfs:domain <http://www.huawei.com/ontology/ietf-network/networks/network> ;
    rdfs:range <http://www.huawei.com/ontology/ietf-network/networks/network/node> ;
    owl:minCardinality 0 .

<http://www.huawei.com/ontology/ietf-network/networks/network/link/destination/dest-node> a owl:ObjectProperty ;
    ex:xpathPath "../../../nw:node/nw:node-id" ;
    rdfs:comment """Destination node identifier.  Must be in the same
network.""" ;
    rdfs:domain <http://www.huawei.com/ontology/ietf-network/networks/network/link/destination> ;
    rdfs:range <http://www.huawei.com/ontology/ietf-network/networks/network> ;
    owl:minCardinality 0 ;
    prov:wasDerivedFrom "nt:link?list/nt:destination?container/nt:dest-node?leaf" .

<http://www.huawei.com/ontology/ietf-network/networks/network/link/destination/dest-tp> a owl:ObjectProperty ;
    ex:xpathPath "../../../nw:node[nw:node-id=current()/../dest-node]/termination-point/tp-id" ;
    rdfs:comment """This termination point is located within the
destination node and terminates the link.""" ;
    rdfs:domain <http://www.huawei.com/ontology/ietf-network/networks/network/link/destination> ;
    rdfs:range <http://www.huawei.com/ontology/ietf-network/networks/network> ;
    owl:minCardinality 0 ;
    prov:wasDerivedFrom "nt:link?list/nt:destination?container/nt:dest-tp?leaf" .

<http://www.huawei.com/ontology/ietf-network/networks/network/link/hasDestination> a owl:ObjectProperty ;
    rdfs:label "hasDestination" ;
    rdfs:comment "Containment relation (parent --> child)." ;
    rdfs:domain <http://www.huawei.com/ontology/ietf-network/networks/network/link> ;
    rdfs:range <http://www.huawei.com/ontology/ietf-network/networks/network/link/destination> ;
    owl:minCardinality 0 ;
    prov:wasDerivedFrom "nt:link?list/hasDestination" .

<http://www.huawei.com/ontology/ietf-network/networks/network/link/hasSource> a owl:ObjectProperty ;
    rdfs:label "hasSource" ;
    rdfs:comment "Containment relation (parent --> child)." ;
    rdfs:domain <http://www.huawei.com/ontology/ietf-network/networks/network/link> ;
    rdfs:range <http://www.huawei.com/ontology/ietf-network/networks/network/link/source> ;
    owl:minCardinality 0 ;
    prov:wasDerivedFrom "nt:link?list/hasSource" .

<http://www.huawei.com/ontology/ietf-network/networks/network/link/hasSupportingLink> a owl:ObjectProperty ;
    rdfs:label "hasSupportingLink" ;
    rdfs:comment "Containment relation (parent --> child)." ;
    rdfs:domain <http://www.huawei.com/ontology/ietf-network/networks/network/link> ;
    rdfs:range <http://www.huawei.com/ontology/ietf-network/networks/network/link/supporting-link> ;
    owl:minCardinality 0 ;
    prov:wasDerivedFrom "nt:link?list/hasSupportingLink" .

<http://www.huawei.com/ontology/ietf-network/networks/network/link/link-id> a owl:DatatypeProperty ;
    rdfs:label "link-id" ;
    rdfs:comment """The identifier of a link in the topology.
A link is specific to a topology to which it belongs.""" ;
    rdfs:domain <http://www.huawei.com/ontology/ietf-network/networks/network/link> ;
    rdfs:range xsd:string ;
    prov:wasDerivedFrom "nt:link?list/nt:link-id?leaf" .

<http://www.huawei.com/ontology/ietf-network/networks/network/link/source/source-node> a owl:ObjectProperty ;
    ex:xpathPath "../../../nw:node/nw:node-id" ;
    rdfs:comment "Source node identifier.  Must be in the same topology." ;
    rdfs:domain <http://www.huawei.com/ontology/ietf-network/networks/network/link/source> ;
    rdfs:range <http://www.huawei.com/ontology/ietf-network/networks/network> ;
    owl:minCardinality 0 ;
    prov:wasDerivedFrom "nt:link?list/nt:source?container/nt:source-node?leaf" .

<http://www.huawei.com/ontology/ietf-network/networks/network/link/source/source-tp> a owl:ObjectProperty ;
    ex:xpathPath "../../../nw:node[nw:node-id=current()/../source-node]/termination-point/tp-id" ;
    rdfs:comment """This termination point is located within the source node
and terminates the link.""" ;
    rdfs:domain <http://www.huawei.com/ontology/ietf-network/networks/network/link/source> ;
    rdfs:range <http://www.huawei.com/ontology/ietf-network/networks/network> ;
    owl:minCardinality 0 ;
    prov:wasDerivedFrom "nt:link?list/nt:source?container/nt:source-tp?leaf" .

<http://www.huawei.com/ontology/ietf-network/networks/network/link/supporting-link/link-ref> a owl:ObjectProperty ;
    rdfs:comment """This leaf identifies a link that is a part
of this link's underlay.  Reference loops in which
a link identifies itself as its underlay, either
directly or transitively, are not allowed.""" ;
    owl:minCardinality 0 ;
    prov:wasDerivedFrom "nt:link?list/nt:supporting-link?list/nt:link-ref?leaf" .

<http://www.huawei.com/ontology/ietf-network/networks/network/link/supporting-link/network-ref> a owl:ObjectProperty ;
    ex:xpathPath "../../../nw:supporting-network/nw:network-ref" ;
    rdfs:comment """This leaf identifies in which underlay topology
the supporting link is present.""" ;
    rdfs:domain <http://www.huawei.com/ontology/ietf-network/networks/network/link/supporting-link> ;
    rdfs:range <http://www.huawei.com/ontology/ietf-network/networks/network> ;
    owl:minCardinality 0 ;
    prov:wasDerivedFrom "nt:link?list/nt:supporting-link?list/nt:network-ref?leaf" .

<http://www.huawei.com/ontology/ietf-network/networks/network/node/hasTerminationPoint> a owl:ObjectProperty ;
    rdfs:label "hasTerminationPoint" ;
    rdfs:comment "Containment relation (parent --> child)." ;
    rdfs:domain <http://www.huawei.com/ontology/ietf-network/networks/network/node> ;
    rdfs:range <http://www.huawei.com/ontology/ietf-network/networks/network/node/termination-point> ;
    owl:minCardinality 0 .

<http://www.huawei.com/ontology/ietf-network/networks/network/node/termination-point/hasSupportingTerminationPoint> a owl:ObjectProperty ;
    rdfs:label "hasSupportingTerminationPoint" ;
    rdfs:comment "Containment relation (parent --> child)." ;
    rdfs:domain <http://www.huawei.com/ontology/ietf-network/networks/network/node/termination-point> ;
    rdfs:range <http://www.huawei.com/ontology/ietf-network/networks/network/node/termination-point/supporting-termination-point> ;
    owl:minCardinality 0 ;
    prov:wasDerivedFrom "nt:termination-point?list/hasSupportingTerminationPoint" .

<http://www.huawei.com/ontology/ietf-network/networks/network/node/termination-point/supporting-termination-point/network-ref> a owl:ObjectProperty ;
    ex:xpathPath "../../../nw:supporting-node/nw:network-ref" ;
    rdfs:comment """This leaf identifies in which topology the
supporting termination point is present.""" ;
    rdfs:domain <http://www.huawei.com/ontology/ietf-network/networks/network/node/termination-point/supporting-termination-point> ;
    rdfs:range <http://www.huawei.com/ontology/ietf-network/networks/network/node> ;
    owl:minCardinality 0 ;
    prov:wasDerivedFrom "nt:termination-point?list/nt:supporting-termination-point?list/nt:network-ref?leaf" .

<http://www.huawei.com/ontology/ietf-network/networks/network/node/termination-point/supporting-termination-point/node-ref> a owl:ObjectProperty ;
    ex:xpathPath "../../../nw:supporting-node/nw:node-ref" ;
    rdfs:comment """This leaf identifies in which node the supporting
termination point is present.""" ;
    rdfs:domain <http://www.huawei.com/ontology/ietf-network/networks/network/node/termination-point/supporting-termination-point> ;
    rdfs:range <http://www.huawei.com/ontology/ietf-network/networks/network/node> ;
    owl:minCardinality 0 ;
    prov:wasDerivedFrom "nt:termination-point?list/nt:supporting-termination-point?list/nt:node-ref?leaf" .

<http://www.huawei.com/ontology/ietf-network/networks/network/node/termination-point/supporting-termination-point/tp-ref> a owl:ObjectProperty ;
    rdfs:comment """Reference to the underlay node (the underlay node must
be in a different topology).""" ;
    owl:minCardinality 0 ;
    prov:wasDerivedFrom "nt:termination-point?list/nt:supporting-termination-point?list/nt:tp-ref?leaf" .

<http://www.huawei.com/ontology/ietf-network/networks/network/node/termination-point/tp-id> a owl:DatatypeProperty ;
    rdfs:label "tp-id" ;
    rdfs:comment "Termination point identifier." ;
    rdfs:domain <http://www.huawei.com/ontology/ietf-network/networks/network/node/termination-point> ;
    rdfs:range xsd:string ;
    prov:wasDerivedFrom "nt:termination-point?list/nt:tp-id?leaf" .

<http://www.huawei.com/ontology/ietf-power-and-energy-txt/energy-objects/hasPowerEntry> a owl:ObjectProperty ;
    rdfs:label "hasPowerEntry" ;
    rdfs:comment "Containment relation (parent --> child)." ;
    rdfs:domain <http://www.huawei.com/ontology/ietf-power-and-energy-txt/energy-objects> ;
    rdfs:range <http://www.huawei.com/ontology/ietf-power-and-energy-txt/energy-objects/power-entry> ;
    owl:minCardinality 0 ;
    prov:wasDerivedFrom "eo:energy-objects?container/hasPowerEntry" .

<http://www.huawei.com/ontology/ietf-power-and-energy-txt/energy-objects/power-entry/eo-power> a owl:DatatypeProperty ;
    rdfs:label "eo-power" ;
    rdfs:comment """The current power usage measurement for the energy object.
This value represents the instantaneous power consumption
of the component. Positive values indicate power
consumption, while negative values can indicate power
generation (e.g., for devices with battery backup or
renewable energy sources).""" ;
    rdfs:domain <http://www.huawei.com/ontology/ietf-power-and-energy-txt/energy-objects/power-entry> ;
    rdfs:range xsd:int ;
    prov:wasDerivedFrom "eo:energy-objects?container/eo:power-entry?list/eo:eo-power?leaf" .

<http://www.huawei.com/ontology/ietf-power-and-energy-txt/energy-objects/power-entry/eo-power-data-source-accuracy> a owl:ObjectProperty ;
    rdfs:label "eo-power-data-source-accuracy" ;
    rdfs:comment """The accuracy of the power data source. Indicates whether
the data source is a direct measurement, an estimate, or
unavailable and also the accuracy level of the data source.
This metadata is crucial for network management
applications to assess the reliability and accuracy of the
power data.""" ;
    rdfs:domain <http://www.huawei.com/ontology/ietf-power-and-energy-txt/energy-objects/power-entry> ;
    rdfs:range <http://www.huawei.com/ontology/identity/data-source-accuracy> ;
    owl:minCardinality 0 ;
    prov:wasDerivedFrom "eo:energy-objects?container/eo:power-entry?list/eo:eo-power-data-source-accuracy?leaf" .

<http://www.huawei.com/ontology/ietf-power-and-energy-txt/energy-objects/power-entry/eo-power-measurement-local> a owl:DatatypeProperty ;
    rdfs:label "eo-power-measurement-local" ;
    rdfs:comment """Indicates whether the power measurement is local (true) or
remote (false). A local measurement is taken directly at
the device, while a remote measurement is collected from
an external source. This information can be useful for
troubleshooting and understanding the data source.""" ;
    rdfs:domain <http://www.huawei.com/ontology/ietf-power-and-energy-txt/energy-objects/power-entry> ;
    rdfs:range xsd:boolean ;
    prov:wasDerivedFrom "eo:energy-objects?container/eo:power-entry?list/eo:eo-power-measurement-local?leaf" .

<http://www.huawei.com/ontology/ietf-power-and-energy-txt/energy-objects/power-entry/eo-power-nameplate> a owl:DatatypeProperty ;
    rdfs:label "eo-power-nameplate" ;
    rdfs:comment """The nameplate power rating of an energy object. This is
the maximum power that the device is designed to consume or
produce, as specified by the manufacturer. Essential for
power budget calculations and capacity planning.""" ;
    rdfs:domain <http://www.huawei.com/ontology/ietf-power-and-energy-txt/energy-objects/power-entry> ;
    rdfs:range xsd:unsignedInt ;
    prov:wasDerivedFrom "eo:energy-objects?container/eo:power-entry?list/eo:eo-power-nameplate?leaf" .

<http://www.huawei.com/ontology/ietf-power-and-energy-txt/energy-objects/power-entry/eo-power-power-factor> a owl:DatatypeProperty ;
    rdfs:label "eo-power-power-factor" ;
    rdfs:comment """The percent value of the power factor measurement for the
energy object. This information is important for
understanding the electrical characteristics of the device
and for correctly interpreting the power data.""" ;
    rdfs:domain <http://www.huawei.com/ontology/ietf-power-and-energy-txt/energy-objects/power-entry> ;
    rdfs:range xsd:unsignedByte ;
    prov:wasDerivedFrom "eo:energy-objects?container/eo:power-entry?list/eo:eo-power-power-factor?leaf" .

<http://www.huawei.com/ontology/ietf-power-and-energy-txt/energy-objects/power-entry/eo-power-unit-multiplier> a owl:ObjectProperty ;
    rdfs:label "eo-power-unit-multiplier" ;
    rdfs:comment """The unit multiplier used to measure the power or energy.
This multiplier applies to both eo-power and
eo-power-nameplate values, allowing representation of power
values from milliwatts to gigawatts using integer
arithmetic.""" ;
    rdfs:domain <http://www.huawei.com/ontology/ietf-power-and-energy-txt/energy-objects/power-entry> ;
    rdfs:range <http://www.huawei.com/ontology/identity/unit-multiplier> ;
    owl:minCardinality 0 ;
    prov:wasDerivedFrom "eo:energy-objects?container/eo:power-entry?list/eo:eo-power-unit-multiplier?leaf" .

<http://www.huawei.com/ontology/ietf-power-and-energy-txt/energy-objects/power-entry/object-id> a owl:DatatypeProperty ;
    rdfs:label "object-id" ;
    rdfs:comment """An identifier that uniquely identifies the energy object
in a device.""" ;
    rdfs:domain <http://www.huawei.com/ontology/ietf-power-and-energy-txt/energy-objects/power-entry> ;
    rdfs:range xsd:string ;
    prov:wasDerivedFrom "eo:energy-objects?container/eo:power-entry?list/eo:object-id?leaf" .

<http://www.huawei.com/ontology/ietf-power-and-energy-txt/energy-objects/power-entry/source-component-id> a owl:ObjectProperty ;
    rdfs:comment """Reference to the component name in the ietf-hardware
model. This leaf creates a direct semantic link between the
power attributes and the physical component they describe.
""" ;
    owl:minCardinality 0 ;
    prov:wasDerivedFrom "eo:energy-objects?container/eo:power-entry?list/eo:source-component-id?leaf" .

ex:ipv4-address a sh:NodeShape ;
    rdfs:label "ipv4-address" ;
    sh:datatype xsd:string ;
    sh:pattern "(([0-9]|[1-9][0-9]|1[0-9][0-9]|2[0-4][0-9]|25[0-5])\\.){3}([0-9]|[1-9][0-9]|1[0-9][0-9]|2[0-4][0-9]|25[0-5])(%[\\p{N}\\p{L}]+)?" .

ex:ipv4-address-no-zone a sh:NodeShape ;
    rdfs:label "ipv4-address-no-zone" ;
    sh:datatype xsd:string ;
    sh:pattern "[0-9\\.]*" .

ex:ipv4-prefix a sh:NodeShape ;
    rdfs:label "ipv4-prefix" ;
    sh:datatype xsd:string ;
    sh:pattern "(([0-9]|[1-9][0-9]|1[0-9][0-9]|2[0-4][0-9]|25[0-5])\\.){3}([0-9]|[1-9][0-9]|1[0-9][0-9]|2[0-4][0-9]|25[0-5])/(([0-9])|([1-2][0-9])|(3[0-2]))" .

ex:ipv6-address a sh:NodeShape ;
    rdfs:label "ipv6-address" ;
    sh:datatype xsd:string ;
    sh:pattern "((:|[0-9a-fA-F]{0,4}):)([0-9a-fA-F]{0,4}:){0,5}((([0-9a-fA-F]{0,4}:)?(:|[0-9a-fA-F]{0,4}))|(((25[0-5]|2[0-4][0-9]|[01]?[0-9]?[0-9])\\.){3}(25[0-5]|2[0-4][0-9]|[01]?[0-9]?[0-9])))(%[\\p{N}\\p{L}]+)?",
        "(([^:]+:){6}(([^:]+:[^:]+)|(.*\\..*)))|((([^:]+:)*[^:]+)?::(([^:]+:)*[^:]+)?)(%.+)?" .

ex:ipv6-address-no-zone a sh:NodeShape ;
    rdfs:label "ipv6-address-no-zone" ;
    sh:datatype xsd:string ;
    sh:pattern "[0-9a-fA-F:\\.]*" .

ex:ipv6-flow-label a sh:NodeShape ;
    rdfs:label "ipv6-flow-label" ;
    sh:datatype xsd:unsignedInt ;
    sh:maxInclusive 1048575 ;
    sh:minInclusive 0 .

ex:ipv6-prefix a sh:NodeShape ;
    rdfs:label "ipv6-prefix" ;
    sh:datatype xsd:string ;
    sh:pattern "((:|[0-9a-fA-F]{0,4}):)([0-9a-fA-F]{0,4}:){0,5}((([0-9a-fA-F]{0,4}:)?(:|[0-9a-fA-F]{0,4}))|(((25[0-5]|2[0-4][0-9]|[01]?[0-9]?[0-9])\\.){3}(25[0-5]|2[0-4][0-9]|[01]?[0-9]?[0-9])))(/(([0-9])|([0-9]{2})|(1[0-1][0-9])|(12[0-8])))",
        "(([^:]+:){6}(([^:]+:[^:]+)|(.*\\..*)))|((([^:]+:)*[^:]+)?::(([^:]+:)*[^:]+)?)(/.+)" .

ex:link-id a sh:NodeShape ;
    rdfs:label "link-id" ;
    sh:datatype xsd:string .

ex:mac-address a sh:NodeShape ;
    rdfs:label "mac-address" ;
    sh:datatype xsd:string ;
    sh:pattern "[0-9a-fA-F]{2}(:[0-9a-fA-F]{2}){5}" .

ex:ne-ref a sh:NodeShape ;
    rdfs:label "ne-ref" ;
    sh:datatype xsd:string .

ex:ni-location-ref a sh:NodeShape ;
    rdfs:label "ni-location-ref" ;
    sh:datatype xsd:string .

<http://www.huawei.com/ontology/notification/hardware-state-change> a owl:Class ;
    rdfs:label "hardware-state-change" .

<http://www.huawei.com/ontology/notification/hardware-state-oper-disabled> a owl:Class ;
    rdfs:label "hardware-state-oper-disabled" .

<http://www.huawei.com/ontology/notification/hardware-state-oper-enabled> a owl:Class ;
    rdfs:label "hardware-state-oper-enabled" .

<http://www.huawei.com/ontology/nwi:network-inventory> a owl:Class .

<http://www.huawei.com/ontology/nwi:network-inventory/nwi:network-elements/nwi:network-element> a owl:Class .

ex:object-identifier a sh:NodeShape ;
    rdfs:label "object-identifier" ;
    sh:datatype xsd:string ;
    sh:pattern "(([0-1](\\.[1-3]?[0-9]))|(2\\.(0|([1-9]\\d*))))(\\.(0|([1-9]\\d*)))*" .

ex:object-identifier-128 a sh:NodeShape ;
    rdfs:label "object-identifier-128" ;
    sh:datatype xsd:string ;
    sh:pattern "\\d*(\\.\\d*){1,127}" .

ex:phys-address a sh:NodeShape ;
    rdfs:label "phys-address" ;
    sh:datatype xsd:string ;
    sh:pattern "([0-9a-fA-F]{2}(:[0-9a-fA-F]{2})*)?" .

ex:port-number a sh:NodeShape ;
    rdfs:label "port-number" ;
    sh:datatype xsd:unsignedShort ;
    sh:maxInclusive 65535 ;
    sh:minInclusive 0 .

<http://www.huawei.com/ontology/power-and-energy-txt/energy-objects/hasPowerEntry> a owl:ObjectProperty ;
    rdfs:label "hasPowerEntry" ;
    rdfs:comment "Containment relation (parent --> child)." ;
    rdfs:domain <http://www.huawei.com/ontology/power-and-energy-txt/energy-objects> ;
    rdfs:range <http://www.huawei.com/ontology/power-and-energy-txt/energy-objects/power-entry> ;
    owl:minCardinality 0 ;
    prov:wasDerivedFrom "eo:energy-objects?container/hasPowerEntry" .

<http://www.huawei.com/ontology/power-and-energy-txt/energy-objects/power-entry/eo-power> a owl:DatatypeProperty ;
    rdfs:label "eo-power" ;
    rdfs:comment """The current power usage measurement for the energy object.
This value represents the instantaneous power consumption
of the component. Positive values indicate power
consumption, while negative values can indicate power
generation (e.g., for devices with battery backup or
renewable energy sources).""" ;
    rdfs:domain <http://www.huawei.com/ontology/power-and-energy-txt/energy-objects/power-entry> ;
    rdfs:range xsd:int ;
    prov:wasDerivedFrom "eo:energy-objects?container/eo:power-entry?list/eo:eo-power?leaf" .

<http://www.huawei.com/ontology/power-and-energy-txt/energy-objects/power-entry/eo-power-data-source-accuracy> a owl:ObjectProperty ;
    rdfs:label "eo-power-data-source-accuracy" ;
    rdfs:comment """The accuracy of the power data source. Indicates whether
the data source is a direct measurement, an estimate, or
unavailable and also the accuracy level of the data source.
This metadata is crucial for network management
applications to assess the reliability and accuracy of the
power data.""" ;
    rdfs:domain <http://www.huawei.com/ontology/power-and-energy-txt/energy-objects/power-entry> ;
    rdfs:range <http://www.huawei.com/ontology/identity/data-source-accuracy> ;
    owl:minCardinality 0 ;
    prov:wasDerivedFrom "eo:energy-objects?container/eo:power-entry?list/eo:eo-power-data-source-accuracy?leaf" .

<http://www.huawei.com/ontology/power-and-energy-txt/energy-objects/power-entry/eo-power-measurement-local> a owl:DatatypeProperty ;
    rdfs:label "eo-power-measurement-local" ;
    rdfs:comment """Indicates whether the power measurement is local (true) or
remote (false). A local measurement is taken directly at
the device, while a remote measurement is collected from
an external source. This information can be useful for
troubleshooting and understanding the data source.""" ;
    rdfs:domain <http://www.huawei.com/ontology/power-and-energy-txt/energy-objects/power-entry> ;
    rdfs:range xsd:boolean ;
    prov:wasDerivedFrom "eo:energy-objects?container/eo:power-entry?list/eo:eo-power-measurement-local?leaf" .

<http://www.huawei.com/ontology/power-and-energy-txt/energy-objects/power-entry/eo-power-nameplate> a owl:DatatypeProperty ;
    rdfs:label "eo-power-nameplate" ;
    rdfs:comment """The nameplate power rating of an energy object. This is
the maximum power that the device is designed to consume or
produce, as specified by the manufacturer. Essential for
power budget calculations and capacity planning.""" ;
    rdfs:domain <http://www.huawei.com/ontology/power-and-energy-txt/energy-objects/power-entry> ;
    rdfs:range xsd:unsignedInt ;
    prov:wasDerivedFrom "eo:energy-objects?container/eo:power-entry?list/eo:eo-power-nameplate?leaf" .

<http://www.huawei.com/ontology/power-and-energy-txt/energy-objects/power-entry/eo-power-power-factor> a owl:DatatypeProperty ;
    rdfs:label "eo-power-power-factor" ;
    rdfs:comment """The percent value of the power factor measurement for the
energy object. This information is important for
understanding the electrical characteristics of the device
and for correctly interpreting the power data.""" ;
    rdfs:domain <http://www.huawei.com/ontology/power-and-energy-txt/energy-objects/power-entry> ;
    rdfs:range xsd:unsignedByte ;
    prov:wasDerivedFrom "eo:energy-objects?container/eo:power-entry?list/eo:eo-power-power-factor?leaf" .

<http://www.huawei.com/ontology/power-and-energy-txt/energy-objects/power-entry/eo-power-unit-multiplier> a owl:ObjectProperty ;
    rdfs:label "eo-power-unit-multiplier" ;
    rdfs:comment """The unit multiplier used to measure the power or energy.
This multiplier applies to both eo-power and
eo-power-nameplate values, allowing representation of power
values from milliwatts to gigawatts using integer
arithmetic.""" ;
    rdfs:domain <http://www.huawei.com/ontology/power-and-energy-txt/energy-objects/power-entry> ;
    rdfs:range <http://www.huawei.com/ontology/identity/unit-multiplier> ;
    owl:minCardinality 0 ;
    prov:wasDerivedFrom "eo:energy-objects?container/eo:power-entry?list/eo:eo-power-unit-multiplier?leaf" .

<http://www.huawei.com/ontology/power-and-energy-txt/energy-objects/power-entry/object-id> a owl:DatatypeProperty ;
    rdfs:label "object-id" ;
    rdfs:comment """An identifier that uniquely identifies the energy object
in a device.""" ;
    rdfs:domain <http://www.huawei.com/ontology/power-and-energy-txt/energy-objects/power-entry> ;
    rdfs:range xsd:string ;
    prov:wasDerivedFrom "eo:energy-objects?container/eo:power-entry?list/eo:object-id?leaf" .

<http://www.huawei.com/ontology/power-and-energy-txt/energy-objects/power-entry/source-component-id> a owl:ObjectProperty ;
    rdfs:comment """Reference to the component name in the ietf-hardware
model. This leaf creates a direct semantic link between the
power attributes and the physical component they describe.
""" ;
    owl:minCardinality 0 ;
    prov:wasDerivedFrom "eo:energy-objects?container/eo:power-entry?list/eo:source-component-id?leaf" .

<http://www.huawei.com/ontology/power-and-energy-txt/hardware> a owl:Class ;
    rdfs:comment """Data nodes representing components.

If the server supports configuration of hardware components,
then this data model is instantiated in the configuration
datastores supported by the server.  The leaf-list 'datastore'
for the module 'ietf-hardware' in the YANG library provides
this information.""" ;
    prov:wasDerivedFrom "hw:hardware?container" .

<http://www.huawei.com/ontology/power-and-energy-txt/network-inventory> a owl:Class ;
    rdfs:comment "Top-level container for network inventory." ;
    prov:wasDerivedFrom "nwi:network-inventory?container" .

ex:power-factor a sh:NodeShape ;
    rdfs:label "power-factor" ;
    sh:datatype xsd:unsignedByte ;
    sh:maxInclusive 100 ;
    sh:minInclusive 0 .

ex:sensor-value a sh:NodeShape ;
    rdfs:label "sensor-value" ;
    sh:datatype xsd:int ;
    sh:maxInclusive 1000000000 ;
    sh:minInclusive -1000000000 .

ex:sensor-value-precision a sh:NodeShape ;
    rdfs:label "sensor-value-precision" ;
    sh:datatype xsd:byte ;
    sh:maxInclusive 9 ;
    sh:minInclusive -8 .

ex:timestamp a sh:NodeShape ;
    rdfs:label "timestamp" ;
    sh:datatype xsd:string .

ex:timeticks a sh:NodeShape ;
    rdfs:label "timeticks" ;
    sh:datatype xsd:unsignedInt .

ex:tp-id a sh:NodeShape ;
    rdfs:label "tp-id" ;
    sh:datatype xsd:string .

<http://www.huawei.com/ontology/types/admin-state/locked> a <http://www.huawei.com/ontology/types/admin-state>,
        owl:NamedIndividual ;
    rdfs:label "locked" ;
    rdfs:comment "The resource is administratively prohibited from use." .

<http://www.huawei.com/ontology/types/admin-state/shutting-down> a <http://www.huawei.com/ontology/types/admin-state>,
        owl:NamedIndividual ;
    rdfs:label "shutting-down" ;
    rdfs:comment """The resource usage is administratively limited to current
instances of use.""" .

<http://www.huawei.com/ontology/types/admin-state/unknown> a <http://www.huawei.com/ontology/types/admin-state>,
        owl:NamedIndividual ;
    rdfs:label "unknown" ;
    rdfs:comment "The resource is unable to report administrative state." .

<http://www.huawei.com/ontology/types/admin-state/unlocked> a <http://www.huawei.com/ontology/types/admin-state>,
        owl:NamedIndividual ;
    rdfs:label "unlocked" ;
    rdfs:comment """The resource is not administratively prohibited from
use.""" .

<http://www.huawei.com/ontology/types/ip-version/ipv4> a <http://www.huawei.com/ontology/types/ip-version>,
        owl:NamedIndividual ;
    rdfs:label "ipv4" ;
    rdfs:comment "The IPv4 protocol as defined in RFC 791." .

<http://www.huawei.com/ontology/types/ip-version/ipv6> a <http://www.huawei.com/ontology/types/ip-version>,
        owl:NamedIndividual ;
    rdfs:label "ipv6" ;
    rdfs:comment "The IPv6 protocol as defined in RFC 2460." .

<http://www.huawei.com/ontology/types/ip-version/unknown> a <http://www.huawei.com/ontology/types/ip-version>,
        owl:NamedIndividual ;
    rdfs:label "unknown" ;
    rdfs:comment """An unknown or unspecified version of the Internet
protocol.""" .

<http://www.huawei.com/ontology/types/oper-state/disabled> a <http://www.huawei.com/ontology/types/oper-state>,
        owl:NamedIndividual ;
    rdfs:label "disabled" ;
    rdfs:comment "The resource is totally inoperable." .

<http://www.huawei.com/ontology/types/oper-state/enabled> a <http://www.huawei.com/ontology/types/oper-state>,
        owl:NamedIndividual ;
    rdfs:label "enabled" ;
    rdfs:comment "The resource is partially or fully operable." .

<http://www.huawei.com/ontology/types/oper-state/testing> a <http://www.huawei.com/ontology/types/oper-state>,
        owl:NamedIndividual ;
    rdfs:label "testing" ;
    rdfs:comment """The resource is currently being tested and cannot
therefore report whether or not it is operational.""" .

<http://www.huawei.com/ontology/types/oper-state/unknown> a <http://www.huawei.com/ontology/types/oper-state>,
        owl:NamedIndividual ;
    rdfs:label "unknown" ;
    rdfs:comment "The resource is unable to report its operational state." .

<http://www.huawei.com/ontology/types/sensor-status/nonoperational> a <http://www.huawei.com/ontology/types/sensor-status>,
        owl:NamedIndividual ;
    rdfs:label "nonoperational" ;
    rdfs:comment """Indicates that the server believes the sensor is broken.
The sensor could have a hard failure (disconnected wire)
or a soft failure such as out-of-range, jittery, or wildly
fluctuating readings.""" .

<http://www.huawei.com/ontology/types/sensor-status/ok> a <http://www.huawei.com/ontology/types/sensor-status>,
        owl:NamedIndividual ;
    rdfs:label "ok" ;
    rdfs:comment "Indicates that the server can obtain the sensor value." .

<http://www.huawei.com/ontology/types/sensor-status/unavailable> a <http://www.huawei.com/ontology/types/sensor-status>,
        owl:NamedIndividual ;
    rdfs:label "unavailable" ;
    rdfs:comment """Indicates that the server presently cannot obtain the
sensor value.""" .

<http://www.huawei.com/ontology/types/sensor-value-scale/atto> a <http://www.huawei.com/ontology/types/sensor-value-scale>,
        owl:NamedIndividual ;
    rdfs:label "atto" ;
    rdfs:comment "Data scaling factor of 10^-18." .

<http://www.huawei.com/ontology/types/sensor-value-scale/exa> a <http://www.huawei.com/ontology/types/sensor-value-scale>,
        owl:NamedIndividual ;
    rdfs:label "exa" ;
    rdfs:comment "Data scaling factor of 10^18." .

<http://www.huawei.com/ontology/types/sensor-value-scale/femto> a <http://www.huawei.com/ontology/types/sensor-value-scale>,
        owl:NamedIndividual ;
    rdfs:label "femto" ;
    rdfs:comment "Data scaling factor of 10^-15." .

<http://www.huawei.com/ontology/types/sensor-value-scale/giga> a <http://www.huawei.com/ontology/types/sensor-value-scale>,
        owl:NamedIndividual ;
    rdfs:label "giga" ;
    rdfs:comment "Data scaling factor of 10^9." .

<http://www.huawei.com/ontology/types/sensor-value-scale/kilo> a <http://www.huawei.com/ontology/types/sensor-value-scale>,
        owl:NamedIndividual ;
    rdfs:label "kilo" ;
    rdfs:comment "Data scaling factor of 10^3." .

<http://www.huawei.com/ontology/types/sensor-value-scale/mega> a <http://www.huawei.com/ontology/types/sensor-value-scale>,
        owl:NamedIndividual ;
    rdfs:label "mega" ;
    rdfs:comment "Data scaling factor of 10^6." .

<http://www.huawei.com/ontology/types/sensor-value-scale/micro> a <http://www.huawei.com/ontology/types/sensor-value-scale>,
        owl:NamedIndividual ;
    rdfs:label "micro" ;
    rdfs:comment "Data scaling factor of 10^-6." .

<http://www.huawei.com/ontology/types/sensor-value-scale/milli> a <http://www.huawei.com/ontology/types/sensor-value-scale>,
        owl:NamedIndividual ;
    rdfs:label "milli" ;
    rdfs:comment "Data scaling factor of 10^-3." .

<http://www.huawei.com/ontology/types/sensor-value-scale/nano> a <http://www.huawei.com/ontology/types/sensor-value-scale>,
        owl:NamedIndividual ;
    rdfs:label "nano" ;
    rdfs:comment "Data scaling factor of 10^-9." .

<http://www.huawei.com/ontology/types/sensor-value-scale/peta> a <http://www.huawei.com/ontology/types/sensor-value-scale>,
        owl:NamedIndividual ;
    rdfs:label "peta" ;
    rdfs:comment "Data scaling factor of 10^15." .

<http://www.huawei.com/ontology/types/sensor-value-scale/pico> a <http://www.huawei.com/ontology/types/sensor-value-scale>,
        owl:NamedIndividual ;
    rdfs:label "pico" ;
    rdfs:comment "Data scaling factor of 10^-12." .

<http://www.huawei.com/ontology/types/sensor-value-scale/tera> a <http://www.huawei.com/ontology/types/sensor-value-scale>,
        owl:NamedIndividual ;
    rdfs:label "tera" ;
    rdfs:comment "Data scaling factor of 10^12." .

<http://www.huawei.com/ontology/types/sensor-value-scale/units> a <http://www.huawei.com/ontology/types/sensor-value-scale>,
        owl:NamedIndividual ;
    rdfs:label "units" ;
    rdfs:comment "Data scaling factor of 10^0." .

<http://www.huawei.com/ontology/types/sensor-value-scale/yocto> a <http://www.huawei.com/ontology/types/sensor-value-scale>,
        owl:NamedIndividual ;
    rdfs:label "yocto" ;
    rdfs:comment "Data scaling factor of 10^-24." .

<http://www.huawei.com/ontology/types/sensor-value-scale/yotta> a <http://www.huawei.com/ontology/types/sensor-value-scale>,
        owl:NamedIndividual ;
    rdfs:label "yotta" ;
    rdfs:comment "Data scaling factor of 10^24." .

<http://www.huawei.com/ontology/types/sensor-value-scale/zepto> a <http://www.huawei.com/ontology/types/sensor-value-scale>,
        owl:NamedIndividual ;
    rdfs:label "zepto" ;
    rdfs:comment "Data scaling factor of 10^-21." .

<http://www.huawei.com/ontology/types/sensor-value-scale/zetta> a <http://www.huawei.com/ontology/types/sensor-value-scale>,
        owl:NamedIndividual ;
    rdfs:label "zetta" ;
    rdfs:comment "Data scaling factor of 10^21." .

<http://www.huawei.com/ontology/types/sensor-value-type/amperes> a <http://www.huawei.com/ontology/types/sensor-value-type>,
        owl:NamedIndividual ;
    rdfs:label "amperes" ;
    rdfs:comment "A measure of electric current." .

<http://www.huawei.com/ontology/types/sensor-value-type/celsius> a <http://www.huawei.com/ontology/types/sensor-value-type>,
        owl:NamedIndividual ;
    rdfs:label "celsius" ;
    rdfs:comment "A measure of temperature." .

<http://www.huawei.com/ontology/types/sensor-value-type/cmm> a <http://www.huawei.com/ontology/types/sensor-value-type>,
        owl:NamedIndividual ;
    rdfs:label "cmm" ;
    rdfs:comment "A measure of cubic meters per minute (airflow)." .

<http://www.huawei.com/ontology/types/sensor-value-type/hertz> a <http://www.huawei.com/ontology/types/sensor-value-type>,
        owl:NamedIndividual ;
    rdfs:label "hertz" ;
    rdfs:comment "A measure of frequency." .

<http://www.huawei.com/ontology/types/sensor-value-type/other> a <http://www.huawei.com/ontology/types/sensor-value-type>,
        owl:NamedIndividual ;
    rdfs:label "other" ;
    rdfs:comment "A measure other than those listed below." .

<http://www.huawei.com/ontology/types/sensor-value-type/percent-RH> a <http://www.huawei.com/ontology/types/sensor-value-type>,
        owl:NamedIndividual ;
    rdfs:label "percent-RH" ;
    rdfs:comment "A measure of percent relative humidity." .

<http://www.huawei.com/ontology/types/sensor-value-type/rpm> a <http://www.huawei.com/ontology/types/sensor-value-type>,
        owl:NamedIndividual ;
    rdfs:label "rpm" ;
    rdfs:comment "A measure of shaft revolutions per minute." .

<http://www.huawei.com/ontology/types/sensor-value-type/truth-value> a <http://www.huawei.com/ontology/types/sensor-value-type>,
        owl:NamedIndividual ;
    rdfs:label "truth-value" ;
    rdfs:comment "Value is one of 1 (true) or 2 (false)" .

<http://www.huawei.com/ontology/types/sensor-value-type/unknown> a <http://www.huawei.com/ontology/types/sensor-value-type>,
        owl:NamedIndividual ;
    rdfs:label "unknown" ;
    rdfs:comment "An unknown measurement or arbitrary, relative numbers" .

<http://www.huawei.com/ontology/types/sensor-value-type/volts-AC> a <http://www.huawei.com/ontology/types/sensor-value-type>,
        owl:NamedIndividual ;
    rdfs:label "volts-AC" ;
    rdfs:comment "A measure of electric potential (alternating current)." .

<http://www.huawei.com/ontology/types/sensor-value-type/volts-DC> a <http://www.huawei.com/ontology/types/sensor-value-type>,
        owl:NamedIndividual ;
    rdfs:label "volts-DC" ;
    rdfs:comment "A measure of electric potential (direct current)." .

<http://www.huawei.com/ontology/types/sensor-value-type/watts> a <http://www.huawei.com/ontology/types/sensor-value-type>,
        owl:NamedIndividual ;
    rdfs:label "watts" ;
    rdfs:comment "A measure of power." .

<http://www.huawei.com/ontology/types/standby-state/cold-standby> a <http://www.huawei.com/ontology/types/standby-state>,
        owl:NamedIndividual ;
    rdfs:label "cold-standby" ;
    rdfs:comment """The resource is to back up another resource, but it will
not be immediately able to take over the role of a
resource to be backed up and will require some
initialization activity.""" .

<http://www.huawei.com/ontology/types/standby-state/hot-standby> a <http://www.huawei.com/ontology/types/standby-state>,
        owl:NamedIndividual ;
    rdfs:label "hot-standby" ;
    rdfs:comment """The resource is not providing service, but it will be
immediately able to take over the role of the resource to
be backed up, without the need for initialization
activity, and will contain the same information as the
resource to be backed up.""" .

<http://www.huawei.com/ontology/types/standby-state/providing-service> a <http://www.huawei.com/ontology/types/standby-state>,
        owl:NamedIndividual ;
    rdfs:label "providing-service" ;
    rdfs:comment "The resource is providing service." .

<http://www.huawei.com/ontology/types/standby-state/unknown> a <http://www.huawei.com/ontology/types/standby-state>,
        owl:NamedIndividual ;
    rdfs:label "unknown" ;
    rdfs:comment "The resource is unable to report standby state." .

<http://www.huawei.com/ontology/types/usage-state/active> a <http://www.huawei.com/ontology/types/usage-state>,
        owl:NamedIndividual ;
    rdfs:label "active" ;
    rdfs:comment """The resource is currently in use, and it has sufficient
spare capacity to provide for additional users.""" .

<http://www.huawei.com/ontology/types/usage-state/busy> a <http://www.huawei.com/ontology/types/usage-state>,
        owl:NamedIndividual ;
    rdfs:label "busy" ;
    rdfs:comment """The resource is currently in use, but it currently has no
spare capacity to provide for additional users.""" .

<http://www.huawei.com/ontology/types/usage-state/idle> a <http://www.huawei.com/ontology/types/usage-state>,
        owl:NamedIndividual ;
    rdfs:label "idle" ;
    rdfs:comment "The resource is servicing no users." .

<http://www.huawei.com/ontology/types/usage-state/unknown> a <http://www.huawei.com/ontology/types/usage-state>,
        owl:NamedIndividual ;
    rdfs:label "unknown" ;
    rdfs:comment "The resource is unable to report usage state." .

ex:uri a sh:NodeShape ;
    rdfs:label "uri" ;
    sh:datatype xsd:string .

ex:uuid a sh:NodeShape ;
    rdfs:label "uuid" ;
    sh:datatype xsd:string ;
    sh:pattern "[0-9a-fA-F]{8}-[0-9a-fA-F]{4}-[0-9a-fA-F]{4}-[0-9a-fA-F]{4}-[0-9a-fA-F]{12}" .

ex:xpath1.0 a sh:NodeShape ;
    rdfs:label "xpath1.0" ;
    sh:datatype xsd:string .

ex:yang-identifier a sh:NodeShape ;
    rdfs:label "yang-identifier" ;
    sh:datatype xsd:string ;
    sh:pattern ".|..|[^xX].*|.[^mM].*|..[^lL].*",
        "[a-zA-Z_][a-zA-Z0-9\\-_.]*" .

ex:zero-based-counter32 a sh:NodeShape ;
    rdfs:label "zero-based-counter32" ;
    sh:datatype xsd:unsignedInt .

ex:zero-based-counter64 a sh:NodeShape ;
    rdfs:label "zero-based-counter64" ;
    sh:datatype xsd:unsignedLong .

<http://www.huawei.com/ontology/identity/accuracy-unknown> a owl:Class,
        owl:NamedIndividual ;
    rdfs:label "accuracy-unknown" ;
    rdfs:comment "The accuracy of the power data is unknown." ;
    rdfs:subClassOf <http://www.huawei.com/ontology/identity/data-source-accuracy> ;
    prov:wasDerivedFrom "eo:accuracy-unknown?identity" .

<http://www.huawei.com/ontology/identity/electrical-cable> a owl:Class,
        owl:NamedIndividual ;
    rdfs:label "electrical-cable" ;
    rdfs:comment "Electrical cable." ;
    rdfs:subClassOf <http://www.huawei.com/ontology/identity/cable-type> ;
    prov:wasDerivedFrom "nwi-passive:electrical-cable?identity" .

<http://www.huawei.com/ontology/ietf-network-inventory-txt/network-inventory> a owl:Class ;
    rdfs:label "network-inventory" ;
    rdfs:comment "Top-level container for network inventory." ;
    prov:wasDerivedFrom "nwi:network-inventory?container" .

<http://www.huawei.com/ontology/ietf-power-and-energy-txt/energy-objects> a owl:Class ;
    rdfs:label "energy-objects" ;
    rdfs:comment "Energy objects container for power attributes." ;
    prov:wasDerivedFrom "eo:energy-objects?container" .

<http://www.huawei.com/ontology/power-and-energy-txt/energy-objects> a owl:Class ;
    rdfs:label "energy-objects" ;
    rdfs:comment "Energy objects container for power attributes." ;
    prov:wasDerivedFrom "eo:energy-objects?container" .

<http://www.huawei.com/ontology/identity/cable-type> a owl:Class,
        owl:NamedIndividual ;
    rdfs:label "cable-type" ;
    rdfs:comment "Base identity for cable types." ;
    prov:wasDerivedFrom "nwi-passive:cable-type?identity" .

<http://www.huawei.com/ontology/identity/connected-device-type> a owl:Class,
        owl:NamedIndividual ;
    rdfs:label "connected-device-type" ;
    rdfs:comment "Base identity for connected device types." ;
    prov:wasDerivedFrom "nwi-passive:connected-device-type?identity" .

<http://www.huawei.com/ontology/identity/ne-type> a owl:Class,
        owl:NamedIndividual ;
    rdfs:label "ne-type" ;
    rdfs:comment "Base identity for network element (NE) types." ;
    prov:wasDerivedFrom "nwi:ne-type?identity" .

<http://www.huawei.com/ontology/identity/unit-multiplier> a owl:Class,
        owl:NamedIndividual ;
    rdfs:label "unit-multiplier" ;
    rdfs:comment """Base identity for unit multipliers as defined in IEC 61850-7-3
Annex A. These represent exponents of 10 for scaling units
associated with the integer units used to measure the power or
energy.""" ;
    prov:wasDerivedFrom "eo:unit-multiplier?identity" .

<http://www.huawei.com/ontology/ietf-hardware/hardware> a owl:Class ;
    rdfs:label "hardware" ;
    rdfs:comment """Data nodes representing components.

If the server supports configuration of hardware components,
then this data model is instantiated in the configuration
datastores supported by the server.  The leaf-list 'datastore'
for the module 'ietf-hardware' in the YANG library provides
this information.""" ;
    prov:wasDerivedFrom "hw:hardware?container" .

<http://www.huawei.com/ontology/ietf-network-inventory-txt/network-inventory/network-elements> a owl:Class ;
    rdfs:label "network-elements" ;
    rdfs:comment """The top-level container for the list of network elements
within the network.""" ;
    prov:wasDerivedFrom "nwi:network-inventory?container/nwi:network-elements?container" .

<http://www.huawei.com/ontology/ietf-network-inventory-txt/network-inventory/network-elements/network-element/components> a owl:Class ;
    rdfs:label "components" ;
    rdfs:comment """The top-level container for the list of components
within a network element.""" ;
    prov:wasDerivedFrom "nwi:network-inventory?container/nwi:network-elements?container/nwi:network-element?list/nwi:components?container" .

<http://www.huawei.com/ontology/ietf-network/networks/network/link/supporting-link> a owl:Class ;
    rdfs:label "supporting-link" ;
    rdfs:comment "Identifies the link or links on which this link depends." ;
    prov:wasDerivedFrom "nt:link?list/nt:supporting-link?list" .

<http://www.huawei.com/ontology/identity/accuracy-estimated> a owl:Class,
        owl:NamedIndividual ;
    rdfs:label "accuracy-estimated" ;
    rdfs:comment """The power data is estimated, perhaps based on a model,
history or calculation rather than a direct measurement.""" ;
    rdfs:subClassOf <http://www.huawei.com/ontology/identity/data-source-accuracy> ;
    prov:wasDerivedFrom "eo:accuracy-estimated?identity" .

<http://www.huawei.com/ontology/ietf-network/networks/network/link/destination> a owl:Class ;
    rdfs:label "destination" ;
    rdfs:comment """This container holds the logical destination of a
particular link.""" ;
    prov:wasDerivedFrom "nt:link?list/nt:destination?container" .

<http://www.huawei.com/ontology/ietf-network/networks/network/link/source> a owl:Class ;
    rdfs:label "source" ;
    rdfs:comment """This container holds the logical source of a particular
link.""" ;
    prov:wasDerivedFrom "nt:link?list/nt:source?container" .

<http://www.huawei.com/ontology/ietf-network/networks/network/node/termination-point> a owl:Class ;
    rdfs:label "termination-point" ;
    rdfs:comment """A termination point can terminate a link.
Depending on the type of topology, a termination point
could, for example, refer to a port or an interface.""" ;
    prov:wasDerivedFrom "nt:termination-point?list" .

<http://www.huawei.com/ontology/ietf-network/networks/network/node/termination-point/supporting-termination-point> a owl:Class ;
    rdfs:label "supporting-termination-point" ;
    rdfs:comment """This list identifies any termination points on which a
given termination point depends or onto which it maps.
Those termination points will themselves be contained
in a supporting node.  This dependency information can be
inferred from the dependencies between links.  Therefore,
this item is not separately configurable.  Hence, no
corresponding constraint needs to be articulated.
The corresponding information is simply provided by the
implementing system.""" ;
    prov:wasDerivedFrom "nt:termination-point?list/nt:supporting-termination-point?list" .

<http://www.huawei.com/ontology/types/ip-version> a owl:Class ;
    rdfs:label "ip-version" .

<http://www.huawei.com/ontology/types/sensor-status> a owl:Class ;
    rdfs:label "sensor-status" .

<http://www.huawei.com/ontology/identity/passive-port-type> a owl:Class,
        owl:NamedIndividual ;
    rdfs:label "passive-port-type" ;
    rdfs:comment "Base identity for passive port types." ;
    prov:wasDerivedFrom "nwi-passive:passive-port-type?identity" .

<http://www.huawei.com/ontology/ietf-network/networks/network/node> a owl:Class .

<http://www.huawei.com/ontology/types/admin-state> a owl:Class ;
    rdfs:label "admin-state" .

<http://www.huawei.com/ontology/types/oper-state> a owl:Class ;
    rdfs:label "oper-state" .

<http://www.huawei.com/ontology/types/standby-state> a owl:Class ;
    rdfs:label "standby-state" .

<http://www.huawei.com/ontology/types/usage-state> a owl:Class ;
    rdfs:label "usage-state" .

<http://www.huawei.com/ontology/identity/accuracy-measured> a owl:Class,
        owl:NamedIndividual ;
    rdfs:label "accuracy-measured" ;
    rdfs:comment """The power data is a direct, real-time measurement
from a sensor.""" ;
    rdfs:subClassOf <http://www.huawei.com/ontology/identity/data-source-accuracy> ;
    prov:wasDerivedFrom "eo:accuracy-measured?identity" .

<http://www.huawei.com/ontology/identity/data-source-accuracy> a owl:Class,
        owl:NamedIndividual ;
    rdfs:label "data-source-accuracy" ;
    rdfs:comment """Base identity for all possible data accuracy types.
This identity serves as the root for a hierarchy of accuracy
types, allowing for extensibility while maintaining alignment
with current and future industry standards.

The hierarchy, as defined in this YANG module, is as follows.
Other modules may extend this hierarchy with additional
accuracy base- and sub-types as needed.

data-source-accuracy
  accuracy-unknown
      accuracy-unavailable
  accuracy-estimated
      accuracy-static
      accuracy-historic
      accuracy-learned
  accuracy-measured
       accuracy-measured-bronze
       accuracy-measured-silver
       accuracy-measured-gold
       accuracy-measured-red
       accuracy-measured-ones
""" ;
    prov:wasDerivedFrom "eo:data-source-accuracy?identity" .

<http://www.huawei.com/ontology/identity/passive-device-type> a owl:Class,
        owl:NamedIndividual ;
    rdfs:label "passive-device-type" ;
    rdfs:comment "Base identity for passive device types." ;
    prov:wasDerivedFrom "nwi-passive:passive-device-type?identity" .

<http://www.huawei.com/ontology/ietf-network-inventory-txt/network-inventory/network-elements/network-element> a owl:Class ;
    rdfs:label "network-element" ;
    rdfs:comment "The list of network elements within the network." ;
    prov:wasDerivedFrom "nwi:network-inventory?container/nwi:network-elements?container/nwi:network-element?list" .

<http://www.huawei.com/ontology/ietf-network-inventory-txt/network-inventory/network-elements/network-element/components/component> a owl:Class ;
    rdfs:label "component" ;
    rdfs:comment "The list of components within a network element." ;
    prov:wasDerivedFrom "nwi:network-inventory?container/nwi:network-elements?container/nwi:network-element?list/nwi:components?container/nwi:component?list" .

<http://www.huawei.com/ontology/ietf-network/networks/network/link> a owl:Class ;
    rdfs:label "link" ;
    rdfs:comment """A network link connects a local (source) node and
a remote (destination) node via a set of the respective
node's termination points.  It is possible to have several
links between the same source and destination nodes.
Likewise, a link could potentially be re-homed between
termination points.  Therefore, in order to ensure that we
would always know to distinguish between links, every link
is identified by a dedicated link identifier.  Note that a
link models a point-to-point link, not a multipoint link.""" ;
    prov:wasDerivedFrom "nt:link?list" .

<http://www.huawei.com/ontology/identity/cable-role> a owl:Class,
        owl:NamedIndividual ;
    rdfs:label "cable-role" ;
    rdfs:comment "Base identity for cable roles." ;
    prov:wasDerivedFrom "nwi-passive:cable-role?identity" .

<http://www.huawei.com/ontology/ietf-hardware/hardware/component/state> a owl:Class ;
    rdfs:label "state" ;
    rdfs:comment "State-related nodes" ;
    prov:wasDerivedFrom "hw:hardware?container/hw:component?list/hw:state?container" .

<http://www.huawei.com/ontology/ietf-network/networks/network> a owl:Class .

<http://www.huawei.com/ontology/ietf-power-and-energy-txt/energy-objects/power-entry> a owl:Class ;
    rdfs:label "power-entry" ;
    rdfs:comment """Power entry for an energy object, indexed by object id.
Each entry contains the complete set of power attributes
for a specific physical component.""" ;
    prov:wasDerivedFrom "eo:energy-objects?container/eo:power-entry?list" .

<http://www.huawei.com/ontology/power-and-energy-txt/energy-objects/power-entry> a owl:Class ;
    rdfs:label "power-entry" ;
    rdfs:comment """Power entry for an energy object, indexed by object id.
Each entry contains the complete set of power attributes
for a specific physical component.""" ;
    prov:wasDerivedFrom "eo:energy-objects?container/eo:power-entry?list" .

<http://www.huawei.com/ontology/ietf-hardware/hardware/component/sensor-data> a owl:Class ;
    rdfs:label "sensor-data" ;
    rdfs:comment """Conditional: exists when derived-from-or-self(../class,
                                   "ianahw:sensor")""",
        "Sensor-related nodes." ;
    prov:wasDerivedFrom "hw:hardware?container/hw:component?list/hw:sensor-data?container" ;
    sh:deactivated """derived-from-or-self(../class,
                                   "ianahw:sensor")""" .

<http://www.huawei.com/ontology/identity/fiber-type> a owl:Class,
        owl:NamedIndividual ;
    rdfs:label "fiber-type" ;
    rdfs:comment "Base identity for fiber types." ;
    prov:wasDerivedFrom "nwi-passive:fiber-type?identity" .

<http://www.huawei.com/ontology/types/sensor-value-type> a owl:Class ;
    rdfs:label "sensor-value-type" .

<http://www.huawei.com/ontology/identity/hardware-class> a owl:Class,
        owl:NamedIndividual ;
    rdfs:label "hardware-class" ;
    rdfs:comment """This identity is the base for all hardware class
identifiers.""" ;
    prov:wasDerivedFrom "ianahw:hardware-class?identity" .

<http://www.huawei.com/ontology/types/sensor-value-scale> a owl:Class ;
    rdfs:label "sensor-value-scale" .

<http://www.huawei.com/ontology/ietf-hardware/hardware/component> a owl:Class ;
    rdfs:label "component" ;
    rdfs:comment """List of components.

When the server detects a new hardware component, it
initializes a list entry in the operational state.

If the server does not support configuration of hardware
components, list entries in the operational state are
initialized with values for all nodes as detected by the
implementation.

Otherwise, this procedure is followed:

  1. If there is an entry in the '/hardware/component' list
     in the intended configuration with values for the nodes
     'class', 'parent', and 'parent-rel-pos' that are equal
     to the detected values, then the list entry in the
     operational state is initialized with the configured
     values, including the 'name'.

  2. Otherwise (i.e., there is no matching configuration
     entry), the list entry in the operational state is
     initialized with values for all nodes as detected by
     the implementation.

If the '/hardware/component' list in the intended
configuration is modified, then the system MUST behave as if
it re-initializes itself and follow the procedure in (1).""" ;
    prov:wasDerivedFrom "hw:hardware?container/hw:component?list" .

